theories/Staging/NewShallow/Executor.v
@@ -28,9 +28,12 @@
 
 From Coq Require Import
      Bool.Bool
+     Classes.Morphisms
+     Classes.RelationClasses
      Lists.List
      NArith.NArith
      Program.Tactics
+     Relations.Relation_Definitions
      Strings.String
      ZArith.BinInt.
 From Equations Require Import
@@ -51,7 +54,19 @@ Import SigTNotations.
 
 Set Implicit Arguments.
 
-Module Type ShallowExecOn
+Local Notation "A ::> R" :=
+  (pointwise_relation A R)
+    (at level 55, right associativity)
+    : signature_scope.
+Local Notation "'∀' x .. y , R " :=
+  (forall_relation (fun x => .. (forall_relation (fun y => R)) ..))
+    (at level 99, x binder, y binder, right associativity,
+      format "'[  ' '[  ' ∀  x  ..  y ']' ,  '/' R ']'")
+    : signature_scope.
+
+Open Scope signature_scope.
+
+Module Type NewShallowExecOn
   (Import B : Base)
   (Import PROG : Program B)
   (Import SIG : Signature B)
@@ -72,152 +87,21 @@ Module Type ShallowExecOn
     Definition CPureSpecM (A : Type) : Type :=
       (A -> L) -> L.
 
-    Definition pure {A : Type} :
-      A -> CPureSpecM A :=
-      fun a POST => POST a.
+    Definition Monotonic {A} : relation (CPureSpecM A) :=
+      (A ::> lentails) ==> lentails.
 
-    Definition map {A B} :
-      (A -> B) -> CPureSpecM A -> CPureSpecM B :=
-      fun f m POST => m (Basics.compose POST f).
+    #[export] Instance monotonic_transitive {A} : Transitive (@Monotonic A).
+    Proof.
+      intros f g h fg gh P Q PQ. transitivity (g Q).
+      apply fg. assumption. apply gh. reflexivity.
+    Qed.
 
-    Definition bind {A B} :
-      CPureSpecM A -> (A -> CPureSpecM B) -> CPureSpecM B :=
-      fun m f POST => m (fun a1 => f a1 POST).
-
-    Local Notation "x <- ma ;; mb" :=
-      (bind ma (fun x => mb))
-        (at level 80, ma at level 90, mb at level 200, right associativity).
-    Local Notation "ma ;; mb" := (bind ma (fun _ => mb)).
-
-    (* For counting the different execution paths of the shallow executor we use
-       different aliases for False and True to distinguish between them. TRUE
-       and FALSE represent execution paths that are pruned, i.e. do not reach
-       the end of a function, and FINISH encodes the successful execution
-       case. *)
-    Definition FALSE : L := lprop False.
-    Definition TRUE : L := lprop True.
-    Definition FINISH : L := lprop True.
-    Global Typeclasses Opaque TRUE.
-    Global Typeclasses Opaque FALSE.
-    Global Typeclasses Opaque FINISH.
-
-    Definition error {A} : CPureSpecM A :=
-      fun POST => FALSE.
-    Definition block {A} : CPureSpecM A :=
-      fun POST => TRUE.
-
-    Definition angelic (σ : Ty) : CPureSpecM (Val σ) :=
-      fun POST => ∃ v : Val σ, POST v.
-
-    Definition angelic_ctx {N : Set} :
-      forall Δ : NCtx N Ty, CPureSpecM (NamedEnv Val Δ) :=
-      fix rec Δ {struct Δ} :=
-        match Δ with
-        | []%ctx  => pure []
-        | Δ ▻ x∷σ => v  <- angelic σ;;
-                     vs <- rec Δ;;
-                     pure (vs ► (x∷σ ↦ v))
-        end.
-    #[global] Arguments angelic_ctx {N} Δ.
-
-    Definition demonic σ : CPureSpecM (Val σ) :=
-      fun POST => ∀ v : Val σ, POST v.
-
-    Definition demonic_ctx {N : Set} :
-      forall Δ : NCtx N Ty, CPureSpecM (NamedEnv Val Δ) :=
-      fix rec Δ {struct Δ} :=
-        match Δ with
-        | []      => pure env.nil
-        | Δ ▻ x∷σ => v  <- demonic σ;;
-                     vs <- rec Δ;;
-                     pure (vs ► (x∷σ ↦ v))
-        end%ctx.
-    #[global] Arguments demonic_ctx {N} Δ.
-
-    Definition assume_formula (fml : Prop) : CPureSpecM unit :=
-      fun POST => !! fml → POST tt.
-
-    Definition assert_formula (fml : Prop) : CPureSpecM unit :=
-      fun POST => !! fml ∧ POST tt.
-
-    (* The paper uses asserted equalities between multiple types, but the
-       symbolic executor can in fact only assert equalities between symbolic
-       terms. We mirror the structure of the symbolic execution and also
-       traverse (the statically known parts) of other data structures. *)
-    Equations(noeqns) assert_eq_env {Δ : Ctx Ty}
-      (δ δ' : Env Val Δ) : CPureSpecM unit :=
-      assert_eq_env env.nil          env.nil            := pure tt;
-      assert_eq_env (env.snoc δ _ t) (env.snoc δ' _ t') :=
-        bind (assert_eq_env δ δ') (fun _ => assert_formula (t = t')).
-
-    Equations(noeqns) assert_eq_nenv {N : Set} {Δ : NCtx N Ty}
-      (δ δ' : NamedEnv Val Δ) : CPureSpecM unit :=
-      assert_eq_nenv env.nil          env.nil            := pure tt;
-      assert_eq_nenv (env.snoc δ _ t) (env.snoc δ' _ t') :=
-        bind (assert_eq_nenv δ δ') (fun _ => assert_formula (t = t')).
-
-    Definition angelic_binary {A} :
-      CPureSpecM A -> CPureSpecM A -> CPureSpecM A :=
-      fun m1 m2 POST =>
-        m1 POST ∨ m2 POST.
-    Definition demonic_binary {A} :
-      CPureSpecM A -> CPureSpecM A -> CPureSpecM A :=
-      fun m1 m2 POST =>
-        m1 POST ∧ m2 POST.
-
-    Definition angelic_list {A} :
-      list A -> CPureSpecM A :=
-      fix rec xs :=
-        match xs with
-        | nil        => error
-        | cons x xs  => angelic_binary (pure x) (rec xs)
-        end.
-
-    Definition demonic_list {A} :
-      list A -> CPureSpecM A :=
-      fix rec xs :=
-        match xs with
-        | nil        => block
-        | cons x xs  => demonic_binary (pure x) (rec xs)
-        end.
-
-    Definition angelic_finite F `{finite.Finite F} :
-      CPureSpecM F :=
-      angelic_list (finite.enum F).
-    #[global] Arguments angelic_finite F {_ _}.
-
-    Definition demonic_finite F `{finite.Finite F} :
-      CPureSpecM F :=
-      demonic_list (finite.enum F).
-    #[global] Arguments demonic_finite F {_ _}.
-
-    Definition angelic_match_bool :
-      Val ty.bool -> CPureSpecM bool :=
-      fun v =>
-        angelic_binary
-          (bind
-             (assert_formula (v = true))
-             (fun _ => pure true))
-          (bind
-             (assert_formula (v = false))
-             (fun _ => pure false)).
-
-    Definition demonic_match_bool :
-      Val ty.bool -> CPureSpecM bool :=
-      fun v =>
-        demonic_binary
-          (bind
-             (assume_formula (v = true))
-             (fun _ => pure true))
-          (bind
-             (assume_formula (v = false))
-             (fun _ => pure false)).
-
-    Local Ltac crush :=
+    Local Ltac solve_wp :=
       repeat
         (try progress subst;
          lazymatch goal with
-         (* These first rules do not change the provability if the goal, i.e. these steps are always complete. *)
+         (* These first rules do not change the provability if the goal, i.e.
+            these steps are always complete. *)
          | x : NamedEnv Val [ctx] |- _ => destruct (env.nilView x)
          | x: NamedEnv Val (_ ▻ _) |- _ => destruct (env.snocView x)
          | |- _ ⊣⊢ _ => split
@@ -235,79 +119,531 @@ Module Type ShallowExecOn
          | H : _ \/ _ |- _ => destruct H
          | |- _ ∨ _ ⊢ _ => apply lor_left
          | |- _ ⊢ _ ∧ _ => apply land_right
-         (* (* Everything below is incomplete. *) *)
+         (* Everything below is incomplete. *)
          | |- _ ⊢ ∃ x : _, _ => eapply lex_right
          | |- (∀ x : _, _) ⊢ _ => eapply lall_left
          | |- _ ⊢ !! ?P  => is_ground P; apply lprop_right; auto; fail
          | _ => easy
          end).
 
-    Lemma wp_angelic_ctx {N : Set} {Δ : NCtx N Ty} (POST : NamedEnv Val Δ -> L) :
-      angelic_ctx Δ POST ⊣⊢ ∃ vs : NamedEnv Val Δ, POST vs.
-    Proof.
-      induction Δ; cbn; cbv [angelic bind pure].
-      - crush.
-      - setoid_rewrite IHΔ. clear IHΔ. crush.
-    Qed.
+    Section Basic.
+      Definition pure {A : Type} :
+        A -> CPureSpecM A :=
+        fun a POST => POST a.
 
-    Lemma wp_demonic_ctx {N : Set} {Δ : NCtx N Ty} (POST : NamedEnv Val Δ -> L) :
-      demonic_ctx Δ POST ⊣⊢ ∀ vs : NamedEnv Val Δ, POST vs.
-    Proof.
-      induction Δ; cbn; cbv [demonic bind pure].
-      - crush.
-      - setoid_rewrite IHΔ. clear IHΔ. crush.
-    Qed.
+      Definition map {A B} :
+        (A -> B) -> CPureSpecM A -> CPureSpecM B :=
+        fun f m POST => m (Basics.compose POST f).
 
-    Lemma wp_angelic_list {A} (xs : list A) (POST : A -> L) :
-      angelic_list xs POST ⊣⊢ ∃ x : A, !! List.In x xs ∧ POST x.
-    Proof.
-      induction xs; cbn; cbv [angelic_binary pure].
-      - setoid_rewrite lfalse_and. now rewrite lex_false.
-      - rewrite IHxs. clear IHxs. repeat crush.
-        apply lor_right2. repeat crush.
-    Qed.
+      Definition bind {A B} :
+        CPureSpecM A -> (A -> CPureSpecM B) -> CPureSpecM B :=
+        fun m f POST => m (fun a1 => f a1 POST).
+      #[global] Arguments bind {A B} ma f _ /.
 
-    Lemma wp_demonic_list {A} (xs : list A) (POST : A -> L) :
-      demonic_list xs POST ⊣⊢ ∀ x : A, !! List.In x xs → POST x.
-    Proof.
-      induction xs; cbn; cbv [demonic_binary pure].
-      - setoid_rewrite limpl_false. now rewrite lall_true.
-      - rewrite IHxs. clear IHxs. split.
-        + repeat crush.
-          apply land_left2. apply (lall_left v).
-            now apply lentails_apply, lprop_right.
-        + apply land_right.
-          * apply (lall_left a), lentails_apply, lprop_right. now left.
-          * apply proper_lall_entails; intros x.
-            apply proper_limpl_entails; [|easy].
-            apply proper_lprop_entails. now right.
-    Qed.
+      (* For counting the different execution paths of the shallow executor we use
+         different aliases for False and True to distinguish between them. TRUE
+         and FALSE represent execution paths that are pruned, i.e. do not reach
+         the end of a function, and FINISH encodes the successful execution
+         case. *)
+      Definition FALSE : L := lprop False.
+      Definition TRUE : L := lprop True.
+      Definition FINISH : L := lprop True.
+      Global Typeclasses Opaque TRUE.
+      Global Typeclasses Opaque FALSE.
+      Global Typeclasses Opaque FINISH.
 
-    Lemma wp_assert_eq_env {Δ : Ctx Ty} (δ δ' : Env Val Δ) :
-      forall POST,
-        assert_eq_env δ δ' POST ⊣⊢ !! (δ = δ') ∧ POST tt.
-    Proof.
-      induction δ; intros POST; env.destroy δ'; cbn;
-        cbv [bind assert_formula pure].
-      - crush.
-      - rewrite IHδ, env.inversion_eq_snoc. clear IHδ.
-        crush; now apply lprop_right.
-    Qed.
+      Definition error {A} : CPureSpecM A :=
+        fun POST => FALSE.
+      Definition block {A} : CPureSpecM A :=
+        fun POST => TRUE.
 
-    Lemma wp_assert_eq_nenv {N} {Δ : NCtx N Ty} (δ δ' : NamedEnv Val Δ) :
-      forall POST,
-        assert_eq_nenv δ δ' POST ⊣⊢ !! (δ = δ') ∧ POST tt.
-    Proof.
-      (* induction δ; intros POST. *)
-      (* - destruct (env.nilView δ'). intuition. *)
-      (* - destruct (env.snocView δ') as [δ']; cbn in *. *)
-      (*   unfold bind, assert_formula. *)
-      (*   now rewrite IHδ, (@env.inversion_eq_snoc _ _ _ b δ δ'). *)
-    Admitted.
+    End Basic.
+    Local Notation "x <- ma ;; mb" :=
+      (bind ma (fun x => mb))
+        (at level 80, ma at level 90, mb at level 200, right associativity).
+    Local Notation "ma ;; mb" := (bind ma (fun _ => mb)).
+
+    Section Nondeterminism.
+
+      Definition angelic (σ : Ty) : CPureSpecM (Val σ) :=
+        fun POST => ∃ v : Val σ, POST v.
+
+      Definition angelic_ctx {N : Set} :
+        forall Δ : NCtx N Ty, CPureSpecM (NamedEnv Val Δ) :=
+        fix rec Δ {struct Δ} :=
+          match Δ with
+          | []%ctx  => pure []
+          | Δ ▻ x∷σ => v  <- angelic σ;;
+                       vs <- rec Δ;;
+                       pure (vs ► (x∷σ ↦ v))
+          end.
+      #[global] Arguments angelic_ctx {N} Δ.
+
+      Definition demonic σ : CPureSpecM (Val σ) :=
+        fun POST => ∀ v : Val σ, POST v.
+
+      Definition demonic_ctx {N : Set} :
+        forall Δ : NCtx N Ty, CPureSpecM (NamedEnv Val Δ) :=
+        fix rec Δ {struct Δ} :=
+          match Δ with
+          | []      => pure env.nil
+          | Δ ▻ x∷σ => v  <- demonic σ;;
+                       vs <- rec Δ;;
+                       pure (vs ► (x∷σ ↦ v))
+          end%ctx.
+      #[global] Arguments demonic_ctx {N} Δ.
+
+      Definition angelic_binary {A} :
+        CPureSpecM A -> CPureSpecM A -> CPureSpecM A :=
+        fun m1 m2 POST =>
+          m1 POST ∨ m2 POST.
+      Definition demonic_binary {A} :
+        CPureSpecM A -> CPureSpecM A -> CPureSpecM A :=
+        fun m1 m2 POST =>
+          m1 POST ∧ m2 POST.
+
+      Definition angelic_list {A} :
+        list A -> CPureSpecM A :=
+        fix rec xs :=
+          match xs with
+          | nil        => error
+          | cons x xs  => angelic_binary (pure x) (rec xs)
+          end.
+
+      Definition demonic_list {A} :
+        list A -> CPureSpecM A :=
+        fix rec xs :=
+          match xs with
+          | nil        => block
+          | cons x xs  => demonic_binary (pure x) (rec xs)
+          end.
+
+      Definition angelic_finite F `{finite.Finite F} :
+        CPureSpecM F :=
+        angelic_list (finite.enum F).
+      #[global] Arguments angelic_finite F {_ _}.
+
+      Definition demonic_finite F `{finite.Finite F} :
+        CPureSpecM F :=
+        demonic_list (finite.enum F).
+      #[global] Arguments demonic_finite F {_ _}.
+
+      Lemma wp_angelic_ctx {N : Set} {Δ : NCtx N Ty} (POST : NamedEnv Val Δ -> L) :
+        angelic_ctx Δ POST ⊣⊢ ∃ vs : NamedEnv Val Δ, POST vs.
+      Proof.
+        induction Δ; cbn; cbv [bind angelic pure].
+        - solve_wp.
+        - setoid_rewrite IHΔ. clear IHΔ. solve_wp.
+      Qed.
+
+      Lemma wp_demonic_ctx {N : Set} {Δ : NCtx N Ty} (POST : NamedEnv Val Δ -> L) :
+        demonic_ctx Δ POST ⊣⊢ ∀ vs : NamedEnv Val Δ, POST vs.
+      Proof.
+        induction Δ; cbn; cbv [demonic bind pure].
+        - solve_wp.
+        - setoid_rewrite IHΔ. clear IHΔ. solve_wp.
+      Qed.
+
+      Lemma wp_angelic_list {A} (xs : list A) (POST : A -> L) :
+        angelic_list xs POST ⊣⊢ ∃ x : A, !! List.In x xs ∧ POST x.
+      Proof.
+        induction xs; cbn; cbv [angelic_binary pure].
+        - setoid_rewrite lfalse_and. now rewrite lex_false.
+        - rewrite IHxs. clear IHxs. repeat solve_wp.
+          apply lor_right2. repeat solve_wp.
+      Qed.
+
+      Lemma wp_demonic_list {A} (xs : list A) (POST : A -> L) :
+        demonic_list xs POST ⊣⊢ ∀ x : A, !! List.In x xs → POST x.
+      Proof.
+        induction xs; cbn; cbv [demonic_binary pure].
+        - setoid_rewrite limpl_false. now rewrite lall_true.
+        - rewrite IHxs. clear IHxs. split.
+          + repeat solve_wp.
+            apply land_left2. apply (lall_left v).
+              now apply lentails_apply, lprop_right.
+          + apply land_right.
+            * apply (lall_left a), lentails_apply, lprop_right. now left.
+            * apply proper_lall_entails; intros x.
+              apply proper_limpl_entails; [|easy].
+              apply proper_lprop_entails. now right.
+      Qed.
+
+    End Nondeterminism.
+
+    Section Guards.
+
+      Definition assume_formula (fml : Prop) : CPureSpecM unit :=
+        fun POST => !! fml → POST tt.
+      #[global] Arguments assume_formula _ _ /.
+      Definition assert_formula (fml : Prop) : CPureSpecM unit :=
+        fun POST => !! fml ∧ POST tt.
+      #[global] Arguments assert_formula _ _ /.
+      Definition produce_chunk (c : SCChunk) : CPureSpecM unit :=
+        fun POST => interpret_scchunk c -∗ POST tt.
+      #[global] Arguments produce_chunk c _ /.
+      Definition consume_chunk (c : SCChunk) : CPureSpecM unit :=
+        fun POST => interpret_scchunk c ∗ POST tt.
+      #[global] Arguments consume_chunk c _/.
+
+      (* The paper uses asserted equalities between multiple types, but the
+         symbolic executor can in fact only assert equalities between symbolic
+         terms. We mirror the structure of the symbolic execution and also
+         traverse (the statically known parts) of other data structures. *)
+      Equations(noeqns) assert_eq_env {Δ : Ctx Ty}
+        (δ δ' : Env Val Δ) : CPureSpecM unit :=
+        assert_eq_env env.nil          env.nil            := pure tt;
+        assert_eq_env (env.snoc δ _ t) (env.snoc δ' _ t') :=
+          bind (assert_eq_env δ δ') (fun _ => assert_formula (t = t')).
+
+      Equations(noeqns) assert_eq_nenv {N : Set} {Δ : NCtx N Ty}
+        (δ δ' : NamedEnv Val Δ) : CPureSpecM unit :=
+        assert_eq_nenv env.nil          env.nil            := pure tt;
+        assert_eq_nenv (env.snoc δ _ t) (env.snoc δ' _ t') :=
+          bind (assert_eq_nenv δ δ') (fun _ => assert_formula (t = t')).
+
+      Lemma wp_assert_formula {F : Prop} (POST : unit -> L) :
+        assert_formula F POST ⊣⊢ (!! F ∧ lemp) ∗ POST tt.
+      Proof. now rewrite lemp_true, land_true, lprop_sep_and. Qed.
+      Lemma wp_assume_formula {F : Prop} (POST : unit -> L) :
+        assume_formula F POST ⊣⊢ ((!! F ∧ lemp) -∗ POST tt).
+      Proof. now rewrite lemp_true, land_true, lprop_wand_impl. Qed.
+
+      Lemma wp_assert_eq_env {Δ : Ctx Ty} (δ δ' : Env Val Δ) :
+        forall POST,
+          assert_eq_env δ δ' POST ⊣⊢ !! (δ = δ') ∧ POST tt.
+      Proof.
+        induction δ; intros POST; env.destroy δ'; cbn;
+          cbv [bind assert_formula pure].
+        - solve_wp.
+        - rewrite IHδ, env.inversion_eq_snoc. clear IHδ.
+          solve_wp; now apply lprop_right.
+      Qed.
+
+      Lemma wp_assert_eq_nenv {N} {Δ : NCtx N Ty} (δ δ' : NamedEnv Val Δ) :
+        forall POST,
+          assert_eq_nenv δ δ' POST ⊣⊢ !! (δ = δ') ∧ POST tt.
+      Proof.
+        unfold NamedEnv.
+        induction δ; intros POST; env.destroy δ'; cbn; cbv [bind assert_formula].
+        - solve_wp.
+        - rewrite IHδ, env.inversion_eq_snoc.
+          rewrite <- lprop_and_distr, land_assoc.
+          solve_wp.
+      Qed.
+
+      (* Lemma monotonic_assert_eq_env {Δ} (δ δ' : Env Val Δ) : *)
+      (*   Proper Monotonic (assert_eq_env δ δ'). *)
+      (* Proof. *)
+      (*   intros P Q PQ. rewrite !wp_assert_eq_env. *)
+      (*   now apply proper_land_entails. *)
+      (* Qed. *)
+
+      (* Lemma monotonic_assert_eq_nenv {N} {Δ : NCtx N Ty} (δ δ' : NamedEnv Val Δ) : *)
+      (*   Proper Monotonic (assert_eq_nenv δ δ'). *)
+      (* Proof. *)
+      (*   intros P Q PQ. rewrite !wp_assert_eq_nenv. *)
+      (*   now apply proper_land_entails. *)
+      (* Qed. *)
+
+    End Guards.
+
+    Section PatternMatching.
+
+      Definition match_bool {A} (v : Val ty.bool) (kt kf : CPureSpecM A) : CPureSpecM A :=
+        fun POST => if v then kt POST else kf POST.
+      #[global] Arguments match_bool {A} v kt kf _ /.
+
+      Definition match_enum {A E} (v : Val (ty.enum E))
+        (cont : enumt E -> CPureSpecM A) : CPureSpecM A :=
+        cont v.
+      #[global] Arguments match_enum {A E} v cont _ /.
+
+      Definition match_sum {A σ τ} (v : Val (ty.sum σ τ))
+        (kinl : Val σ -> CPureSpecM A) (kinr : Val τ -> CPureSpecM A) :
+        CPureSpecM A :=
+        fun POST =>
+          match v with
+          | inl v1 => kinl v1 POST
+          | inr v2 => kinr v2 POST
+          end.
+      #[global] Arguments match_sum {A σ τ} v kinl kinr _ /.
+
+      Definition match_prod {A σ τ} (v : Val (ty.prod σ τ)) (k : Val σ -> Val τ -> CPureSpecM A) : CPureSpecM A :=
+        fun POST =>
+          match v with
+          | pair v1 v2 => k v1 v2 POST
+          end.
+      #[global] Arguments match_prod {A σ τ} v k _ /.
+
+      Definition match_list {A σ} (v : Val (ty.list σ)) (knil : CPureSpecM A)
+        (kcons : Val σ -> Val (ty.list σ) -> CPureSpecM A) :
+        CPureSpecM A :=
+        fun POST =>
+          match v with
+          | nil       => knil POST
+          | cons x xs => kcons x xs POST
+          end.
+      #[global] Arguments match_list {A σ} v knil kcons _ /.
+
+      Definition match_record {N : Set} {A R} {Δ : NCtx N Ty} (p : RecordPat (recordf_ty R) Δ)
+        (v : Val (ty.record R)) (k : NamedEnv Val Δ -> CPureSpecM A) :
+        CPureSpecM A := k (record_pattern_match_val p v).
+      #[global] Arguments match_record {_ _ _ _} p v k _ /.
+
+      Definition match_tuple {N : Set} {A σs} {Δ : NCtx N Ty}
+        (p : TuplePat σs Δ) (v : Val (ty.tuple σs))
+        (k : NamedEnv Val Δ -> CPureSpecM A) :
+        CPureSpecM A := k (tuple_pattern_match_val p v).
+      #[global] Arguments match_tuple {_ _ _ _} p v k _ /.
+
+      Definition match_union {N : Set} {A U} {Δ : unionk U -> NCtx N Ty}
+        (p : forall K : unionk U, Pattern (Δ K) (unionk_ty U K)) (v : Val (ty.union U))
+        (k : forall K, NamedEnv Val (Δ K) -> CPureSpecM A) : CPureSpecM A :=
+        fun POST =>
+          let (UK , vf) := unionv_unfold U v in
+          k UK (pattern_match_val (p UK) vf) POST.
+      #[global] Arguments match_union {_ _ _ _} p v k _ /.
+
+      Definition match_bvec {A n} (v : Val (ty.bvec n))
+        (k : bv n -> CPureSpecM A) : CPureSpecM A :=
+        k v.
+      #[global] Arguments match_bvec {_ _} v k _ /.
+
+      Definition match_bvec_split {A m n} (v : Val (ty.bvec (m + n)))
+        (k : bv m -> bv n -> CPureSpecM A) : CPureSpecM A :=
+        fun POST =>
+          match bv.appView m n v with
+          | bv.isapp xs ys => k xs ys POST
+          end.
+      #[global] Arguments match_bvec_split {_ _ _} v k _ /.
+
+    End PatternMatching.
+
+    Section ProduceConsume.
+
+      Fixpoint produce {Σ} (ι : Valuation Σ) (asn : Assertion Σ) : CPureSpecM unit :=
+        match asn with
+        | asn.formula fml => assume_formula (inst fml ι)
+        | asn.chunk c     => produce_chunk (inst c ι)
+        | asn.chunk_angelic c => produce_chunk (inst c ι)
+        | asn.match_bool b a1 a2  => match_bool (inst b ι) (produce ι a1) (produce ι a2)
+        | asn.match_enum E k alts =>
+          match_enum
+            (inst (T := fun Σ => Term Σ _) k ι)
+            (fun K => produce ι (alts K))
+        | asn.match_sum σ τ s xl alt_inl xr alt_inr =>
+          match_sum
+            (inst (T := fun Σ => Term Σ _) s ι)
+            (fun v => produce (env.snoc ι (xl∷σ) v) alt_inl)
+            (fun v => produce (env.snoc ι (xr∷τ) v) alt_inr)
+        | asn.match_list s alt_nil xh xt alt_cons =>
+          match_list
+            (inst (T := fun Σ => Term Σ _) s ι)
+            (produce ι alt_nil)
+            (fun vh vt => produce (ι ► (xh∷_ ↦ vh) ► (xt∷ty.list _ ↦ vt)) alt_cons)
+        | asn.match_prod s xl xr rhs =>
+          match_prod
+            (inst (T := fun Σ => Term Σ _) s ι)
+            (fun vl vr => produce (ι ► (xl∷_ ↦ vl) ► (xr∷_ ↦ vr)) rhs)
+        | asn.match_tuple s p rhs =>
+          match_tuple p
+            (inst (T := fun Σ => Term Σ _) s ι)
+            (fun ι' => produce (ι ►► ι') rhs)
+        | asn.match_record R s p rhs =>
+          match_record p
+            (inst (T := fun Σ => Term Σ _) s ι)
+            (fun ι' => produce (ι ►► ι') rhs)
+        | asn.match_union U s alt__ctx alt__pat alt__rhs =>
+          match_union
+            alt__pat (inst (T := fun Σ => Term Σ _) s ι)
+            (fun UK ι' => produce (ι ►► ι') (alt__rhs UK))
+        | asn.sep a1 a2   => _ <- produce ι a1 ;; produce ι a2
+        | asn.or a1 a2 =>
+          demonic_binary (produce ι a1)
+                         (produce ι a2)
+        | asn.exist ς τ a =>
+          v <- demonic τ ;;
+          produce (env.snoc ι (ς∷τ) v) a
+        | asn.debug => pure tt
+        end.
+
+      Fixpoint consume {Σ} (ι : Valuation Σ) (asn : Assertion Σ) : CPureSpecM unit :=
+        match asn with
+        | asn.formula fml => assert_formula (inst fml ι)
+        | asn.chunk c     => consume_chunk (inst c ι)
+        | asn.chunk_angelic c     => consume_chunk (inst c ι)
+        | asn.match_bool b a1 a2  => match_bool (inst b ι) (consume ι a1) (consume ι a2)
+        | asn.match_enum E k alts =>
+          match_enum
+            (inst (T := fun Σ => Term Σ _) k ι)
+            (fun K => consume ι (alts K))
+        | asn.match_sum σ τ s xl alt_inl xr alt_inr =>
+          match_sum
+            (inst (T := fun Σ => Term Σ _) s ι)
+            (fun v => consume (env.snoc ι (xl∷σ) v) alt_inl)
+            (fun v => consume (env.snoc ι (xr∷τ) v) alt_inr)
+        | asn.match_list s alt_nil xh xt alt_cons =>
+          match_list
+            (inst (T := fun Σ => Term Σ _) s ι)
+            (consume ι alt_nil)
+            (fun vh vt => consume (ι ► (xh∷_ ↦ vh) ► (xt∷ty.list _ ↦ vt)) alt_cons)
+        | asn.match_prod s xl xr rhs =>
+          match_prod
+            (inst (T := fun Σ => Term Σ _) s ι)
+            (fun vl vr => consume (ι ► (xl∷_ ↦ vl) ► (xr∷_ ↦ vr)) rhs)
+        | asn.match_tuple s p rhs =>
+          match_tuple p
+            (inst (T := fun Σ => Term Σ _) s ι)
+            (fun ι' => consume (ι ►► ι') rhs)
+        | asn.match_record R s p rhs =>
+          match_record p
+            (inst (T := fun Σ => Term Σ _) s ι)
+            (fun ι' => consume (ι ►► ι') rhs)
+        | asn.match_union U s alt__ctx alt__pat alt__rhs =>
+          match_union
+            alt__pat (inst (T := fun Σ => Term Σ _) s ι)
+            (fun UK ι' => consume (ι ►► ι') (alt__rhs UK))
+        | asn.sep a1 a2   => _ <- consume ι a1;; consume ι a2
+        | asn.or a1 a2 =>
+          angelic_binary (consume ι a1)
+                         (consume ι a2)
+        | asn.exist ς τ a =>
+          v <- angelic τ ;;
+          consume (env.snoc ι (ς∷τ) v) a
+        | asn.debug => pure tt
+        end.
+
+      Lemma wp_produce {Σ} {ι : Valuation Σ} {asn : Assertion Σ} (POST : unit -> L) :
+        produce ι asn POST ⊣⊢ (asn.interpret asn ι -∗ POST tt).
+      Proof.
+        revert POST. induction asn; cbn - [inst inst_term]; intros POST.
+        - apply wp_assume_formula.
+        - unfold produce_chunk; now rewrite interpret_scchunk_inst.
+        - unfold produce_chunk; now rewrite interpret_scchunk_inst.
+        - destruct (inst b ι); cbn; auto.
+        - apply H.
+        - destruct (inst s ι); cbn; auto.
+        - destruct (inst s ι); cbn; auto.
+        - destruct (inst s ι); cbn; auto.
+        - auto.
+        - auto.
+        - destruct (unionv_unfold U (inst s ι)); auto.
+        - now rewrite IHasn1, IHasn2, lwand_curry.
+        - unfold demonic_binary. now rewrite IHasn1, IHasn2, lwand_disj_distr.
+        - unfold demonic. rewrite lwand_exists_comm.
+          now apply proper_lall_equiv.
+        - now rewrite lwand_emp.
+      Qed.
+
+      Lemma wp_consume {Σ} {ι : Valuation Σ} {asn : Assertion Σ} (POST : unit -> L) :
+        consume ι asn POST ⊣⊢ asn.interpret asn ι ∗ POST tt.
+      Proof.
+        revert POST. induction asn; cbn - [inst inst_term]; intros POST.
+        - apply wp_assert_formula.
+        - unfold consume_chunk; now rewrite interpret_scchunk_inst.
+        - unfold consume_chunk; now rewrite interpret_scchunk_inst.
+        - destruct (inst b ι); cbn; auto.
+        - apply H.
+        - destruct (inst s ι); cbn; auto.
+        - destruct (inst s ι); cbn; auto.
+        - destruct (inst s ι); cbn; auto.
+        - auto.
+        - auto.
+        - destruct (unionv_unfold U (inst s ι)); auto.
+        - now rewrite IHasn1, IHasn2, <- lsep_assoc.
+        - rewrite lsep_disj_distr. now apply proper_lor_equiv.
+        - rewrite lsep_exists_comm. now apply proper_lex_equiv.
+        - now rewrite lsep_comm, lsep_emp.
+      Qed.
+
+    End ProduceConsume.
+
+    Section Calls.
+
+      Definition call_contract {Δ τ} (ctr : SepContract Δ τ) (args : CStore Δ) :
+        CPureSpecM (Val τ) :=
+          match ctr with
+          | MkSepContract _ _ Σe δ req result ens =>
+            ι <- angelic_ctx Σe ;;
+            assert_eq_nenv args (inst δ ι) ;;
+            consume ι req  ;;
+            v <- demonic τ ;;
+            produce (env.snoc ι (result∷τ) v) ens ;;
+            pure v
+          end.
+
+      Definition call_contract' {Δ τ} (ctr : SepContract Δ τ) (args : CStore Δ) :
+        CPureSpecM (Val τ) :=
+        fun POST =>
+          match ctr with
+          | MkSepContract _ _ Σe δ req result ens =>
+              ∃ ι : Valuation Σe, !! (args = inst δ ι) ∧
+              asn.interpret req ι ∗ (∀ v : Val τ, asn.interpret ens ι.[result∷τ ↦ v] -∗ POST v)
+          end.
+
+      Definition call_lemma {Δ} (lem : Lemma Δ) (args : CStore Δ) : CPureSpecM unit :=
+          match lem with
+          | MkLemma _ Σe δ req ens =>
+            ι <- angelic_ctx Σe ;;
+            assert_eq_nenv args (inst δ ι) ;;
+            consume ι req ;;
+            produce ι ens
+          end.
+
+      Definition call_lemma' {Δ} (lem : Lemma Δ) (args : CStore Δ) : CPureSpecM (Val ty.unit) :=
+        fun POST =>
+          match lem with
+          | MkLemma _ Σe δ req ens =>
+              ∃ ι : Valuation Σe, !! (args = inst δ ι) ∧
+              asn.interpret req ι ∗ (asn.interpret ens ι -∗ POST tt)
+          end.
+
+      Lemma equiv_call_contract {Δ τ} (ctr : SepContract Δ τ) (args : CStore Δ) :
+        forall (POST : Val τ -> L),
+          call_contract ctr args POST ⊣⊢ call_contract' ctr args POST.
+      Proof.
+        intros POST; destruct ctr as [Σe δΔ req res ens].
+        cbv [call_contract call_contract' bind demonic].
+        rewrite wp_angelic_ctx. apply proper_lex_equiv. intros ι.
+        rewrite wp_assert_eq_nenv. apply proper_land_equiv; [easy|].
+        rewrite wp_consume. apply proper_lsep_equiv; [easy|].
+        apply proper_lall_equiv. intros v.
+        apply wp_produce.
+      Qed.
+
+      Lemma equiv_call_lemma {Δ} (lem : Lemma Δ) (args : CStore Δ) :
+        forall (POST : Val ty.unit -> L),
+        call_lemma lem args POST ⊣⊢ call_lemma' lem args POST.
+      Proof.
+        intros POST; destruct lem as [Σe δΔ req ens].
+        cbv [call_lemma call_lemma' bind demonic].
+        rewrite wp_angelic_ctx. apply proper_lex_equiv. intros ι.
+        rewrite wp_assert_eq_nenv. apply proper_land_equiv; [easy|].
+        rewrite wp_consume. apply proper_lsep_equiv; [easy|].
+        apply wp_produce.
+      Qed.
+
+      Instance monotonic_call_contract {Δ τ} (ctr : SepContract Δ τ) (args : CStore Δ) :
+        Proper Monotonic (call_contract ctr args).
+      Proof.
+        intros P Q PQ. rewrite !equiv_call_contract.
+        destruct ctr; cbn. now setoid_rewrite PQ.
+      Qed.
+
+      Instance monotonic_call_lemma {Δ} (lem : Lemma Δ) (args : CStore Δ) :
+        Proper Monotonic (call_lemma lem args).
+      Proof.
+        intros P Q PQ. rewrite !equiv_call_lemma.
+        destruct lem; cbn. now setoid_rewrite PQ.
+      Qed.
+
+    End Calls.
 
   End WithProp.
   End CPureSpecM.
   Export CPureSpecM (CPureSpecM).
+  #[export] Hint Unfold CPureSpecM.Monotonic : typeclass_instances.
 
   Module CHeapSpecM.
   Section WithProp.
@@ -324,16 +660,19 @@ Module Type ShallowExecOn
 
     Section Basic.
 
-      Definition lift_purem {Γ} {A : Type} :
-        @CPureSpecM L A -> CHeapSpecM Γ Γ A :=
-        fun m POST δ => m (fun a => POST a δ).
+      Definition lift_purem {Γ A} (m : CPureSpecM A) : CHeapSpecM Γ Γ A :=
+        fun POST δ => m (fun a => POST a δ).
+      #[global] Arguments lift_purem {Γ A} m _ /.
 
       Definition pure {Γ A} (a : A) : CHeapSpecM Γ Γ A :=
         fun POST => POST a.
+      #[global] Arguments pure {_ _} a _ /.
       Definition bind {Γ1 Γ2 Γ3 A B} (ma : CHeapSpecM Γ1 Γ2 A) (f : A -> CHeapSpecM Γ2 Γ3 B) : CHeapSpecM Γ1 Γ3 B :=
         fun POST => ma (fun a => f a POST).
+      #[global] Arguments bind {_ _ _ _ _} ma f _ /.
       Definition bind_right {Γ1 Γ2 Γ3 A B} (ma : CHeapSpecM Γ1 Γ2 A) (mb : CHeapSpecM Γ2 Γ3 B) : CHeapSpecM Γ1 Γ3 B :=
         bind ma (fun _ => mb).
+      #[global] Arguments bind_right {_ _ _ _ _} ma mb _ /.
       Definition map {Γ1 Γ2 A B} (f : A -> B) (ma : CHeapSpecM Γ1 Γ2 A) : CHeapSpecM Γ1 Γ2 B :=
         fun POST => ma (fun a => POST (f a)).
 
@@ -341,6 +680,7 @@ Module Type ShallowExecOn
         fun POST δ => ⊥.
       Definition block {Γ1 Γ2 A} : CHeapSpecM Γ1 Γ2 A :=
         fun POST δ => ⊤.
+      #[global] Arguments block {_ _ _} _ /.
 
       Definition demonic_binary {Γ1 Γ2 A} (m1 m2 : CHeapSpecM Γ1 Γ2 A) : CHeapSpecM Γ1 Γ2 A :=
         fun POST δ => m1 POST δ ∧ m2 POST δ.
@@ -351,28 +691,7 @@ Module Type ShallowExecOn
         fun POST δ => ∀ v : Val σ, POST v δ.
       Definition angelic {Γ} (σ : Ty) : CHeapSpecM Γ Γ (Val σ) :=
         fun POST δ => ∃ v : Val σ, POST v δ.
-
-      Definition angelic_ctx {N : Set} {Γ} :
-        forall Δ : NCtx N Ty, CHeapSpecM Γ Γ (NamedEnv Val Δ) :=
-        fun Δ => lift_purem (CPureSpecM.angelic_ctx Δ).
-      #[global] Arguments angelic_ctx {N Γ} Δ.
-
-      Definition angelic_list {A Γ} (xs : list A) : CHeapSpecM Γ Γ A :=
-        lift_purem (CPureSpecM.angelic_list xs).
-
-      Definition angelic_finite F `{finite.Finite F} {Γ} : CHeapSpecM Γ Γ F :=
-        lift_purem (CPureSpecM.angelic_finite F).
-      #[global] Arguments angelic_finite F {_ _ Γ}.
-
-      Definition demonic_finite F `{finite.Finite F} {Γ} : CHeapSpecM Γ Γ F :=
-        lift_purem (CPureSpecM.demonic_finite F).
-      #[global] Arguments demonic_finite F {_ _ Γ}.
-
-      Definition demonic_ctx {N : Set} {Γ} :
-        forall Δ : NCtx N Ty, CHeapSpecM Γ Γ (NamedEnv Val Δ) :=
-        fun Δ => lift_purem (CPureSpecM.demonic_ctx Δ).
-      #[global] Arguments demonic_ctx {N Γ} Δ.
-
+      #[global] Arguments angelic {Γ} σ _ /.
     End Basic.
     #[local] Notation "x <- ma ;; mb" :=
         (bind ma (fun x => mb))
@@ -380,24 +699,6 @@ Module Type ShallowExecOn
     #[local] Notation "ma ;; mb" := (bind_right ma mb) : mut_scope.
     #[local] Infix "⊗" := demonic_binary (at level 40, left associativity) : mut_scope.
     #[local] Infix "⊕" := angelic_binary (at level 50, left associativity) : mut_scope.
-
-    Opaque CHeapSpecM.
-    Opaque lift_purem.
-    Opaque pure.
-    Opaque bind.
-    Opaque bind_right.
-    Opaque map.
-    Opaque error.
-    Opaque block.
-    Opaque demonic_binary.
-    Opaque angelic_binary.
-    Opaque demonic.
-    Opaque angelic.
-    Opaque angelic_ctx.
-    Opaque angelic_list.
-    Opaque angelic_finite.
-    Opaque demonic_finite.
-    Opaque demonic_ctx.
 
     (* Module CHeapSpecMNotations. *)
 
@@ -418,481 +719,76 @@ Module Type ShallowExecOn
     (* Import CHeapSpecMNotations. *)
     (* Local Open Scope mut_scope. *)
 
-    Section AssumeAssert.
-
-      Definition assume_formula {Γ} (fml : Prop) : CHeapSpecM Γ Γ unit :=
-        lift_purem (CPureSpecM.assume_formula fml).
-      Definition assert_formula {Γ} (fml : Prop) : CHeapSpecM Γ Γ unit :=
-        lift_purem (CPureSpecM.assert_formula fml).
-      Definition assert_eq_env {Γ} {Δ : Ctx Ty} (δ δ' : Env Val Δ) : CHeapSpecM Γ Γ unit :=
-        lift_purem (CPureSpecM.assert_eq_env δ δ').
-      Definition assert_eq_nenv {N Γ} {Δ : NCtx N Ty} (δ δ' : NamedEnv Val Δ) : CHeapSpecM Γ Γ unit :=
-        lift_purem (CPureSpecM.assert_eq_nenv δ δ').
-      Definition produce_chunk {Γ} (c : SCChunk) : CHeapSpecM Γ Γ unit :=
-        fun POST δ => interpret_scchunk c -∗ POST tt δ.
-      Definition consume_chunk {Γ} (c : SCChunk) : CHeapSpecM Γ Γ unit :=
-        fun POST δ => interpret_scchunk c ∗ POST tt δ.
-      #[global] Arguments produce_chunk {Γ} _.
-      #[global] Arguments consume_chunk {Γ} _.
-
-    End AssumeAssert.
-
     Section PatternMatching.
 
-      Definition angelic_match_bool {A Γ1 Γ2} (v : Val ty.bool) (kt kf : CHeapSpecM Γ1 Γ2 A) : CHeapSpecM Γ1 Γ2 A :=
-        (assert_formula (v = true);; kt) ⊕ (assert_formula (v = false);; kf).
+      Definition match_bool {A Γ1 Γ2} (v : Val ty.bool) (kt kf : CHeapSpecM Γ1 Γ2 A) : CHeapSpecM Γ1 Γ2 A :=
+        fun POST δ => if v then kt POST δ else kf POST δ.
+      #[global] Arguments match_bool {_ _ _} v kt kf _ /.
 
-      Lemma wp_angelic_match_bool {A Γ1 Γ2} (v : Val ty.bool) (kt kf : CHeapSpecM Γ1 Γ2 A) :
-        forall POST δ,
-          angelic_match_bool v kt kf POST δ ⊣⊢
-          if v then kt POST δ else kf POST δ.
-      Proof.
-        (* cbv [angelic_match_bool angelic_binary bind_right bind assert_formula *)
-        (*      lift_purem CPureSpecM.assert_formula is_true negb]. *)
-        (* destruct v; intuition; discriminate. *)
-      Admitted.
-
-      Definition demonic_match_bool {A Γ1 Γ2} (v : Val ty.bool) (kt kf : CHeapSpecM Γ1 Γ2 A) : CHeapSpecM Γ1 Γ2 A :=
-        (assume_formula (v = true);; kt) ⊗ (assume_formula (v = false);; kf).
-
-      Lemma wp_demonic_match_bool {A Γ1 Γ2} (v : Val ty.bool) (kt kf : CHeapSpecM Γ1 Γ2 A) :
-        forall POST δ,
-          demonic_match_bool v kt kf POST δ ⊣⊢
-          if v then kt POST δ else kf POST δ.
-      Proof.
-        (* cbv [demonic_match_bool demonic_binary bind_right bind assume_formula *)
-        (*      lift_purem CPureSpecM.assume_formula is_true negb]. *)
-        (* destruct v; intuition; discriminate. *)
-      Admitted.
-
-      Definition angelic_match_enum {A E} {Γ1 Γ2} (v : Val (ty.enum E))
+      Definition match_enum {A E} {Γ1 Γ2} (v : Val (ty.enum E))
         (cont : enumt E -> CHeapSpecM Γ1 Γ2 A) : CHeapSpecM Γ1 Γ2 A :=
-        EK <- angelic_finite (enumt E);;
-        assert_formula (v = EK);;
-        cont EK.
+        cont v.
+      #[global] Arguments match_enum {_ _ _ _} v cont _ /.
 
-      Definition demonic_match_enum {A E} {Γ1 Γ2} (v : Val (ty.enum E))
-        (cont : enumt E -> CHeapSpecM Γ1 Γ2 A) : CHeapSpecM Γ1 Γ2 A :=
-        EK <- demonic_finite (enumt E);;
-        assume_formula (v = EK);;
-        cont EK.
-
-      Lemma wp_angelic_match_enum {A E Γ1 Γ2} (v : Val (ty.enum E)) (k : enumt E -> CHeapSpecM Γ1 Γ2 A) :
-        forall POST δ,
-          angelic_match_enum v k POST δ ⊣⊢ k v POST δ.
-      Proof.
-        (* cbv [assert_formula bind bind_right angelic_match_enum angelic_finite *)
-        (*      lift_purem CPureSpecM.angelic_finite CPureSpecM.assert_formula]. *)
-        (* intros. rewrite CPureSpecM.wp_angelic_list. *)
-        (* split; intros; destruct_conjs; subst; auto. *)
-        (* exists v. split; auto. *)
-        (* rewrite <- base.elem_of_list_In. *)
-        (* apply finite.elem_of_enum. *)
-      Admitted.
-
-      Lemma wp_demonic_match_enum {A E Γ1 Γ2} (v : Val (ty.enum E)) (k : enumt E -> CHeapSpecM Γ1 Γ2 A) :
-        forall POST δ,
-          demonic_match_enum v k POST δ ⊣⊢ k v POST δ.
-      Proof.
-        (* cbv [assume_formula bind bind_right demonic_match_enum demonic_finite *)
-        (*      lift_purem CPureSpecM.demonic_finite CPureSpecM.assume_formula]. *)
-        (* intros. rewrite CPureSpecM.wp_demonic_list. *)
-        (* split; intros; subst; auto. *)
-        (* apply H; auto. *)
-        (* rewrite <- base.elem_of_list_In. *)
-        (* apply finite.elem_of_enum. *)
-      Admitted.
-
-      Definition angelic_match_sum {A Γ1 Γ2} {σ τ} (v : Val (ty.sum σ τ))
+      Definition match_sum {A Γ1 Γ2} {σ τ} (v : Val (ty.sum σ τ))
         (kinl : Val σ -> CHeapSpecM Γ1 Γ2 A) (kinr : Val τ -> CHeapSpecM Γ1 Γ2 A) :
         CHeapSpecM Γ1 Γ2 A :=
-        (v1 <- angelic σ;; assert_formula (inl v1 = v);; kinl v1) ⊕
-        (v1 <- angelic τ;; assert_formula (inr v1 = v);; kinr v1).
+        fun POST δ =>
+          match v with
+          | inl v1 => kinl v1 POST δ
+          | inr v2 => kinr v2 POST δ
+          end.
+      #[global] Arguments match_sum {_ _ _ _ _} v kinl kinr _ /.
 
-      Definition demonic_match_sum {A Γ1 Γ2} {σ τ} (v : Val (ty.sum σ τ))
-        (kinl : Val σ -> CHeapSpecM Γ1 Γ2 A) (kinr : Val τ -> CHeapSpecM Γ1 Γ2 A) :
-        CHeapSpecM Γ1 Γ2 A :=
-        (v1 <- demonic σ;; assume_formula (inl v1 = v);; kinl v1) ⊗
-        (v1 <- demonic τ;; assume_formula (inr v1 = v);; kinr v1).
+      Definition match_prod {A Γ1 Γ2} {σ τ} (v : Val (ty.prod σ τ)) (k : Val σ -> Val τ -> CHeapSpecM Γ1 Γ2 A) : CHeapSpecM Γ1 Γ2 A :=
+        fun POST δ =>
+          match v with
+          | pair v1 v2 => k v1 v2 POST δ
+          end.
+      #[global] Arguments match_prod {_ _ _ _ _} v k _ /.
 
-      Lemma wp_angelic_match_sum {A Γ1 Γ2} {σ τ}
-        (v : Val (ty.sum σ τ)) (kinl : Val σ -> CHeapSpecM Γ1 Γ2 A) (kinr : Val τ -> CHeapSpecM Γ1 Γ2 A) POST δ :
-        angelic_match_sum v kinl kinr POST δ ⊣⊢
-        match v with
-        | inl v => kinl v POST δ
-        | inr v => kinr v POST δ
-        end.
-      Proof.
-        (* cbv [angelic_match_sum bind_right bind angelic angelic_binary *)
-        (*      assert_formula lift_purem CPureSpecM.assert_formula]. *)
-        (* split. *)
-        (* - intros []; destruct_conjs; subst; auto. *)
-        (* - destruct v as [v|v]; [left|right]; exists v; intuition. *)
-      Admitted.
-
-      Lemma wp_demonic_match_sum {A Γ1 Γ2} {σ τ}
-        (v : Val (ty.sum σ τ)) (kinl : Val σ -> CHeapSpecM Γ1 Γ2 A) (kinr : Val τ -> CHeapSpecM Γ1 Γ2 A) POST δ :
-        demonic_match_sum v kinl kinr POST δ ⊣⊢
-        match v with
-        | inl v => kinl v POST δ
-        | inr v => kinr v POST δ
-        end.
-      Proof.
-        (* cbv [demonic_match_sum bind_right bind demonic demonic_binary *)
-        (*      assume_formula lift_purem CPureSpecM.assume_formula]. *)
-        (* split. *)
-        (* - destruct v; intuition. *)
-        (* - destruct v; intuition; try discriminate; *)
-        (*     match goal with *)
-        (*     | H: inl _ = inl _ |- _ => apply noConfusion_inv in H; cbn in H; subst *)
-        (*     | H: inr _ = inr _ |- _ => apply noConfusion_inv in H; cbn in H; subst *)
-        (*     end; auto. *)
-      Admitted.
-
-      Definition angelic_match_prod {A Γ1 Γ2} {σ τ} :
-        Val (ty.prod σ τ) -> (Val σ -> Val τ -> CHeapSpecM Γ1 Γ2 A) -> CHeapSpecM Γ1 Γ2 A :=
-        fun v k =>
-          v1 <- angelic σ ;;
-          v2 <- angelic τ ;;
-          assert_formula ((v1,v2) = v) ;;
-          k v1 v2.
-
-      Lemma wp_angelic_match_prod {A Γ1 Γ2} {σ τ}
-        (v : Val (ty.prod σ τ)) (k : Val σ -> Val τ -> CHeapSpecM Γ1 Γ2 A) POST δ :
-        angelic_match_prod v k POST δ ⊣⊢
-        match v with
-        | pair v1 v2 => k v1 v2 POST δ
-        end.
-      Proof.
-        (* cbv [angelic_match_prod bind_right bind angelic angelic_binary *)
-        (*      assert_formula lift_purem CPureSpecM.assert_formula]. *)
-        (* destruct v; intuition. *)
-        (* - destruct H as (v1 & v2 & eq & H). *)
-        (*   inversion eq; now subst. *)
-        (* - now exists v, v0. *)
-      Admitted.
-
-      Definition demonic_match_prod {A Γ1 Γ2} {σ τ} :
-        Val (ty.prod σ τ) -> (Val σ -> Val τ -> CHeapSpecM Γ1 Γ2 A) -> CHeapSpecM Γ1 Γ2 A :=
-        fun v k =>
-          v1 <- demonic σ ;;
-          v2 <- demonic τ ;;
-          assume_formula ((v1,v2) = v) ;;
-          k v1 v2.
-
-      Lemma wp_demonic_match_prod {A Γ1 Γ2} {σ τ}
-        (v : Val (ty.prod σ τ)) (k : Val σ -> Val τ -> CHeapSpecM Γ1 Γ2 A) POST δ :
-        demonic_match_prod v k POST δ ⊣⊢
-        match v with
-        | pair v1 v2 => k v1 v2 POST δ
-        end.
-      Proof.
-        (* cbv [demonic_match_prod bind_right bind demonic demonic_binary *)
-        (*      assume_formula lift_purem CPureSpecM.assume_formula]. *)
-        (* destruct v; intuition. *)
-      Admitted.
-
-      Definition angelic_match_list {A Γ1 Γ2} {σ} (v : Val (ty.list σ))
+      Definition match_list {A Γ1 Γ2} {σ} (v : Val (ty.list σ))
         (knil : CHeapSpecM Γ1 Γ2 A)
         (kcons : Val σ -> Val (ty.list σ) -> CHeapSpecM Γ1 Γ2 A) :
         CHeapSpecM Γ1 Γ2 A :=
-        (assert_formula (nil = v);; knil) ⊕
-        (vhead <- angelic σ;;
-         vtail <- angelic (ty.list σ);;
-         assert_formula (cons vhead vtail = v);;
-         kcons vhead vtail).
+        fun POST δ =>
+          match v with
+          | nil => knil POST δ
+          | cons x xs => kcons x xs POST δ
+          end.
+      #[global] Arguments match_list {_ _ _ _} v knil kcons _ /.
 
-      Lemma wp_angelic_match_list {A Γ1 Γ2} {σ}
-        (v : Val (ty.list σ)) (knil : CHeapSpecM Γ1 Γ2 A) (kcons : Val σ -> Val (ty.list σ) -> CHeapSpecM Γ1 Γ2 A) POST δ :
-        angelic_match_list v knil kcons POST δ ⊣⊢
-        match v with
-        | nil => knil POST δ
-        | cons vh vt => kcons vh vt POST δ
-        end.
-      Proof.
-        (* cbv [angelic_match_list bind_right bind angelic angelic_binary *)
-        (*      assert_formula lift_purem CPureSpecM.assert_formula]. *)
-        (* split. *)
-        (* - intros []; destruct_conjs; subst; auto. *)
-        (* - destruct v as [|vh vt]; [left;auto|right]. *)
-        (*   exists vh, vt. auto. *)
-      Admitted.
+      Definition match_record {N : Set} {A R Γ1 Γ2} {Δ : NCtx N Ty} (p : RecordPat (recordf_ty R) Δ)
+        (v : Val (ty.record R)) (k : NamedEnv Val Δ -> CHeapSpecM Γ1 Γ2 A) :
+        CHeapSpecM Γ1 Γ2 A := k (record_pattern_match_val p v).
+      #[global] Arguments match_record {_ _ _ _ _ _} p v k _ /.
 
-      Definition demonic_match_list {A Γ1 Γ2} {σ} (v : Val (ty.list σ))
-        (knil : CHeapSpecM Γ1 Γ2 A)
-        (kcons : Val σ -> Val (ty.list σ) -> CHeapSpecM Γ1 Γ2 A) :
-        CHeapSpecM Γ1 Γ2 A :=
-        (assume_formula (nil = v);; knil) ⊗
-        (vhead <- demonic σ;;
-         vtail <- demonic (ty.list σ);;
-         assume_formula (cons vhead vtail = v);;
-         kcons vhead vtail).
+      Definition match_tuple {N : Set} {A σs Γ1 Γ2} {Δ : NCtx N Ty}
+        (p : TuplePat σs Δ) (v : Val (ty.tuple σs))
+        (k : NamedEnv Val Δ -> CHeapSpecM Γ1 Γ2 A) :
+        CHeapSpecM Γ1 Γ2 A := k (tuple_pattern_match_val p v).
+      #[global] Arguments match_tuple {_ _ _ _ _ _} p v k _ /.
 
-      Lemma wp_demonic_match_list {A Γ1 Γ2} {σ}
-        (v : Val (ty.list σ)) (knil : CHeapSpecM Γ1 Γ2 A) (kcons : Val σ -> Val (ty.list σ) -> CHeapSpecM Γ1 Γ2 A) POST δ :
-        demonic_match_list v knil kcons POST δ ⊣⊢
-        match v with
-        | nil => knil POST δ
-        | cons vh vt => kcons vh vt POST δ
-        end.
-      Proof.
-        (* cbv [demonic_match_list bind_right bind demonic demonic_binary *)
-        (*      assume_formula lift_purem CPureSpecM.assume_formula]. *)
-        (* split. *)
-        (* - destruct v; intuition. *)
-        (* - destruct v; intuition; try discriminate. *)
-      Admitted.
+      Definition match_union {N : Set} {A Γ1 Γ2 U} {Δ : unionk U -> NCtx N Ty}
+        (p : forall K : unionk U, Pattern (Δ K) (unionk_ty U K)) (v : Val (ty.union U))
+        (k : forall K, NamedEnv Val (Δ K) -> CHeapSpecM Γ1 Γ2 A) : CHeapSpecM Γ1 Γ2 A :=
+        fun POST δ =>
+          let (UK , vf) := unionv_unfold U v in
+          k UK (pattern_match_val (p UK) vf) POST δ.
+      #[global] Arguments match_union {_ _ _ _ _ _} p v k _ /.
 
-      Definition angelic_match_record {N : Set} {A R Γ1 Γ2} {Δ : NCtx N Ty} (p : RecordPat (recordf_ty R) Δ) :
-        (Val (ty.record R)) ->
-        (NamedEnv Val Δ -> CHeapSpecM Γ1 Γ2 A) ->
-        CHeapSpecM Γ1 Γ2 A :=
-        fun v k =>
-          args <- angelic_ctx Δ ;;
-          assert_formula (recordv_fold R (record_pattern_match_env_reverse p args) = v) ;;
-          k args.
+      Definition match_bvec {A n} {Γ1 Γ2} (v : Val (ty.bvec n))
+        (k : bv n -> CHeapSpecM Γ1 Γ2 A) : CHeapSpecM Γ1 Γ2 A :=
+        k v.
+      #[global] Arguments match_bvec {_ _ _ _} v k _ /.
 
-      Lemma wp_angelic_match_record {N : Set} {A R Γ1 Γ2} {Δ : NCtx N Ty} (p : RecordPat (recordf_ty R) Δ)
-        (v : Val (ty.record R)) (k : NamedEnv Val Δ -> CHeapSpecM Γ1 Γ2 A) POST δ :
-        angelic_match_record p v k POST δ ⊣⊢
-        k (record_pattern_match_val p v) POST δ.
-      Proof.
-        (* cbv [angelic_match_record bind_right bind angelic_ctx lift_purem assert_formula CPureSpecM.assert_formula]. *)
-        (* rewrite CPureSpecM.wp_angelic_ctx; intuition. *)
-        (* - destruct H as (vs & <- & H). *)
-        (*   unfold record_pattern_match_val. *)
-        (*   now rewrite recordv_unfold_fold, record_pattern_match_env_inverse_right. *)
-        (* - exists (record_pattern_match_val p v). *)
-        (*   unfold record_pattern_match_val. *)
-        (*   now rewrite record_pattern_match_env_inverse_left, recordv_fold_unfold. *)
-      Admitted.
-
-      Definition demonic_match_record {N : Set} {A R Γ1 Γ2} {Δ : NCtx N Ty} (p : RecordPat (recordf_ty R) Δ) :
-        (Val (ty.record R)) ->
-        (NamedEnv Val Δ -> CHeapSpecM Γ1 Γ2 A) ->
-        CHeapSpecM Γ1 Γ2 A :=
-        fun v k =>
-          args <- demonic_ctx Δ ;;
-          assume_formula (recordv_fold R (record_pattern_match_env_reverse p args) = v) ;;
-          k args.
-
-      Lemma wp_demonic_match_record {N : Set} {A R Γ1 Γ2} {Δ : NCtx N Ty} (p : RecordPat (recordf_ty R) Δ)
-        (v : Val (ty.record R))
-        (k : NamedEnv Val Δ -> CHeapSpecM Γ1 Γ2 A)
-        POST δ :
-        demonic_match_record p v k POST δ ⊣⊢
-        k (record_pattern_match_val p v) POST δ.
-      Proof.
-        (* cbv [demonic_match_record bind_right bind demonic_ctx lift_purem assume_formula CPureSpecM.assume_formula]. *)
-        (* rewrite CPureSpecM.wp_demonic_ctx; intuition; eauto. *)
-        (* eapply H. *)
-        (* - unfold record_pattern_match_val. *)
-        (*   now rewrite record_pattern_match_env_inverse_left, recordv_fold_unfold. *)
-        (* - unfold record_pattern_match_val in H. *)
-        (*   replace (record_pattern_match_env p (recordv_unfold R v)) with vs in H; [assumption|]. *)
-        (*   subst. *)
-        (*   now rewrite recordv_unfold_fold, record_pattern_match_env_inverse_right. *)
-      Admitted.
-
-      Definition angelic_match_tuple {N : Set} {A σs Γ1 Γ2} {Δ : NCtx N Ty} (p : TuplePat σs Δ) :
-        (Val (ty.tuple σs)) ->
-        (NamedEnv Val Δ -> CHeapSpecM Γ1 Γ2 A) ->
-        CHeapSpecM Γ1 Γ2 A :=
-        fun v k =>
-          args <- angelic_ctx Δ ;;
-          assert_formula (tuple_pattern_match_val p v = args) ;;
-          k args.
-
-      Lemma wp_angelic_match_tuple {N : Set} {A σs Γ1 Γ2} {Δ : NCtx N Ty} (p : TuplePat σs Δ)
-        (v : Val (ty.tuple σs)) (k : NamedEnv Val Δ -> CHeapSpecM Γ1 Γ2 A) POST δ :
-        angelic_match_tuple p v k POST δ ⊣⊢
-        k (tuple_pattern_match_val p v) POST δ.
-      Proof.
-        (* cbv [angelic_match_tuple bind_right bind angelic_ctx lift_purem assert_formula CPureSpecM.assert_formula]. *)
-        (* rewrite CPureSpecM.wp_angelic_ctx; intuition. *)
-        (* - now destruct H as (vs & <- & H). *)
-        (* - exists (tuple_pattern_match_val p v). *)
-        (*   split; auto. *)
-      Admitted.
-
-      Definition demonic_match_tuple {N : Set} {A σs Γ1 Γ2} {Δ : NCtx N Ty} (p : TuplePat σs Δ) :
-        (Val (ty.tuple σs)) ->
-        (NamedEnv Val Δ -> CHeapSpecM Γ1 Γ2 A) ->
-        CHeapSpecM Γ1 Γ2 A :=
-        fun v k =>
-          args <- demonic_ctx Δ ;;
-          assume_formula (tuple_pattern_match_val p v = args) ;;
-          k args.
-
-      Lemma wp_demonic_match_tuple {N : Set} {A σs Γ1 Γ2} {Δ : NCtx N Ty} (p : TuplePat σs Δ)
-        (v : Val (ty.tuple σs)) (k : NamedEnv Val Δ -> CHeapSpecM Γ1 Γ2 A) POST δ :
-        demonic_match_tuple p v k POST δ ⊣⊢
-        k (tuple_pattern_match_val p v) POST δ.
-      Proof.
-        (* cbv [demonic_match_tuple bind_right bind demonic_ctx lift_purem assume_formula CPureSpecM.assume_formula]. *)
-        (* rewrite CPureSpecM.wp_demonic_ctx; intuition; subst; auto. *)
-      Admitted.
-
-      Definition angelic_match_pattern {N : Set} {σ} {Δ : NCtx N Ty}
-        (p : Pattern Δ σ) {Γ} (v : Val σ) : CHeapSpecM Γ Γ (NamedEnv Val Δ) :=
-        vs <- angelic_ctx Δ ;;
-        assert_formula (pattern_match_val p v = vs) ;;
-        pure vs.
-
-      Lemma wp_angelic_match_pattern {N : Set} {σ Γ} {Δ : NCtx N Ty} (p : Pattern Δ σ)
-        (v : Val σ) POST δ :
-        angelic_match_pattern (Γ := Γ) p v POST δ ⊣⊢
-        POST (pattern_match_val p v) δ.
-      Proof.
-        (* cbv [angelic_match_pattern bind pure angelic_ctx assert_formula *)
-        (*      lift_purem CPureSpecM.assert_formula]. *)
-        (* rewrite CPureSpecM.wp_angelic_ctx. *)
-        (* split. *)
-        (* - now intros (vs & <- & H). *)
-        (* - intros ?. exists (pattern_match_val p v). *)
-        (*   split; auto. *)
-      Admitted.
-
-      Definition demonic_match_pattern {N : Set} {σ} {Δ : NCtx N Ty}
-        (p : Pattern Δ σ) {Γ} (v : Val σ) : CHeapSpecM Γ Γ (NamedEnv Val Δ) :=
-        vs <- demonic_ctx Δ ;;
-        assume_formula (pattern_match_val p v = vs) ;;
-        pure vs.
-
-      Lemma wp_demonic_match_pattern {N : Set} {σ Γ} {Δ : NCtx N Ty} (p : Pattern Δ σ)
-        (v : Val σ) POST δ :
-        demonic_match_pattern (Γ := Γ) p v POST δ ⊣⊢
-        POST (pattern_match_val p v) δ.
-      Proof.
-        (* cbv [demonic_match_pattern bind pure demonic_ctx bind_right assume_formula *)
-        (*      lift_purem CPureSpecM.assume_formula]. *)
-        (* rewrite CPureSpecM.wp_demonic_ctx. *)
-        (* intuition; subst; auto. *)
-      Admitted.
-
-      Definition angelic_match_union {N : Set} {A Γ1 Γ2 U}
-        {Δ : unionk U -> NCtx N Ty} (p : forall K : unionk U, Pattern (Δ K) (unionk_ty U K)) :
-        Val (ty.union U) -> (forall K, NamedEnv Val (Δ K) -> CHeapSpecM Γ1 Γ2 A) -> CHeapSpecM Γ1 Γ2 A :=
-        fun v POST =>
-          UK     <- angelic_finite (unionk U);;
-          v__field <- angelic (unionk_ty U UK);;
-          assert_formula (unionv_fold U (existT UK v__field) = v);;
-          x      <- angelic_match_pattern (p UK) v__field;;
-          POST UK x.
-
-      Lemma wp_angelic_match_union {N : Set} {A Γ1 Γ2 U}
-        {Δ : unionk U -> NCtx N Ty} (p : forall K : unionk U, Pattern (Δ K) (unionk_ty U K))
-        (v : Val (ty.union U)) (k : forall K, NamedEnv Val (Δ K) -> CHeapSpecM Γ1 Γ2 A)
-        POST δ :
-        angelic_match_union p v k POST δ ⊣⊢
-        let (UK , vf) := unionv_unfold U v in
-        k UK (pattern_match_val (p UK) vf) POST δ.
-      Proof.
-        (* cbv [angelic_match_union bind bind_right angelic_finite assert_formula angelic *)
-        (*      lift_purem CPureSpecM.angelic_finite CPureSpecM.assert_formula]. *)
-        (* rewrite CPureSpecM.wp_angelic_list. *)
-        (* split. *)
-        (* - intros (UK & HIn & vf & Heq & Hwp). *)
-        (*   rewrite wp_angelic_match_pattern in Hwp. *)
-        (*   subst v. now rewrite unionv_unfold_fold. *)
-        (* - destruct (unionv_unfold U v) as [UK vf] eqn:Heq. *)
-        (*   intros Hwp. *)
-        (*   exists UK. split. *)
-        (*   rewrite <- base.elem_of_list_In. *)
-        (*   apply finite.elem_of_enum. *)
-        (*   exists vf. rewrite <- Heq. *)
-        (*   rewrite wp_angelic_match_pattern. *)
-        (*   rewrite unionv_fold_unfold. split; auto. *)
-      Admitted.
-
-      Definition demonic_match_union {N : Set} {A Γ1 Γ2 U}
-        {Δ : unionk U -> NCtx N Ty} (p : forall K : unionk U, Pattern (Δ K) (unionk_ty U K)) :
-        Val (ty.union U) -> (forall K, NamedEnv Val (Δ K) -> CHeapSpecM Γ1 Γ2 A) -> CHeapSpecM Γ1 Γ2 A :=
-        fun v POST =>
-          UK     <- demonic_finite (unionk U);;
-          v__field <- demonic (unionk_ty U UK);;
-          assume_formula (unionv_fold U (existT UK v__field) = v);;
-          x      <- demonic_match_pattern (p UK) v__field;;
-          POST UK x.
-
-      Lemma wp_demonic_match_union {N : Set} {A Γ1 Γ2 U}
-        {Δ : unionk U -> NCtx N Ty} (p : forall K : unionk U, Pattern (Δ K) (unionk_ty U K))
-        (v : Val (ty.union U)) (k : forall K, NamedEnv Val (Δ K) -> CHeapSpecM Γ1 Γ2 A)
-        POST δ :
-        demonic_match_union p v k POST δ ⊣⊢
-        let (UK , vf) := unionv_unfold U v in
-        k UK (pattern_match_val (p UK) vf) POST δ.
-      Proof.
-        (* cbv [demonic_match_union bind bind_right demonic_finite assume_formula demonic *)
-        (*      lift_purem CPureSpecM.demonic_finite CPureSpecM.assume_formula]. *)
-        (* rewrite CPureSpecM.wp_demonic_list. *)
-        (* split. *)
-        (* - destruct (unionv_unfold U v) as [UK vf] eqn:Heq. *)
-        (*   intros HYP. specialize (HYP UK). *)
-        (*   inster HYP by *)
-        (*       rewrite <- base.elem_of_list_In; apply finite.elem_of_enum. *)
-        (*   specialize (HYP vf). *)
-        (*   rewrite wp_demonic_match_pattern in HYP. *)
-        (*   apply HYP. *)
-        (*   now rewrite <- Heq, unionv_fold_unfold. *)
-        (* - intros HYP UK HIn vf <-. *)
-        (*   rewrite unionv_unfold_fold in HYP. *)
-        (*   now rewrite wp_demonic_match_pattern. *)
-      Admitted.
-
-      Definition demonic_match_bvec {A n} {Γ1 Γ2} :
-        Val (ty.bvec n) -> (bv n -> CHeapSpecM Γ1 Γ2 A) -> CHeapSpecM Γ1 Γ2 A :=
-        fun v POST =>
-          u <- demonic_finite (bv n);;
-          assume_formula (v = u);;
-          POST u.
-      #[global] Arguments demonic_match_bvec : simpl never.
-
-      Lemma wp_demonic_match_bvec {A n Γ1 Γ2} (v : Val (ty.bvec n)) (k : bv n -> CHeapSpecM Γ1 Γ2 A) :
-        forall POST δ,
-          demonic_match_bvec v k POST δ ⊣⊢ k v POST δ.
-      Proof.
-        (* cbv [assume_formula bind bind_right demonic_match_bvec demonic_finite *)
-        (*      lift_purem CPureSpecM.demonic_finite CPureSpecM.assume_formula]. *)
-        (* intros. rewrite CPureSpecM.wp_demonic_list. *)
-        (* split; intros; subst; auto. *)
-        (* apply H; auto. *)
-        (* rewrite <- base.elem_of_list_In. *)
-        (* apply finite.elem_of_enum. *)
-      Admitted.
-
-      Definition demonic_match_bvec_split {A m n} {Γ1 Γ2} :
-        Val (ty.bvec (m + n)) ->
-        (bv m -> bv n -> CHeapSpecM Γ1 Γ2 A) -> CHeapSpecM Γ1 Γ2 A :=
-        fun v POST =>
-          v1 <- demonic (ty.bvec m) ;;
-          v2 <- demonic (ty.bvec n) ;;
-          assume_formula (bv.app v1 v2 = v) ;;
-          POST v1 v2.
-      #[global] Arguments demonic_match_bvec_split : simpl never.
-
-      Lemma wp_demonic_match_bvec_split {A m n Γ1 Γ2}
-        (v : Val (ty.bvec (m + n))) (k : bv m -> bv n -> CHeapSpecM Γ1 Γ2 A) :
-        forall POST δ,
-          demonic_match_bvec_split v k POST δ ⊣⊢
+      Definition match_bvec_split {A m n} {Γ1 Γ2} (v : Val (ty.bvec (m + n)))
+        (k : bv m -> bv n -> CHeapSpecM Γ1 Γ2 A) : CHeapSpecM Γ1 Γ2 A :=
+        fun POST δ =>
           match bv.appView m n v with
           | bv.isapp xs ys => k xs ys POST δ
           end.
-      Proof.
-        intros POST δ.
-        cbv [demonic_match_bvec_split bind demonic bind_right
-           assume_formula lift_purem CPureSpecM.assume_formula].
-        destruct (bv.appView m n v) as [v1 v2].
-        split.
-        - apply (lall_left v1).
-          apply (lall_left v2).
-          apply lentails_apply.
-          now apply lprop_right.
-        - apply lall_right; intros v1'.
-          apply lall_right; intros v2'.
-          apply lprop_intro_impl; intros [H1 H2]%bv.app_inj.
-          now subst.
-      Qed.
+      #[global] Arguments match_bvec_split {_ _ _ _ _} v k _ /.
 
     End PatternMatching.
 
@@ -901,141 +797,31 @@ Module Type ShallowExecOn
       Definition pushpop {A Γ1 Γ2 x σ} (v : Val σ)
         (d : CHeapSpecM (Γ1 ▻ x∷σ) (Γ2 ▻ x∷σ) A) : CHeapSpecM Γ1 Γ2 A :=
         fun POST δ0 => d (fun a δ1 => POST a (env.tail δ1)) (δ0 ► (x∷σ ↦ v)).
+      #[global] Arguments pushpop {_ _ _ _ _} v d _ /.
       Definition pushspops {A} {Γ1 Γ2 Δ} (δΔ : CStore Δ)
         (d : CHeapSpecM (Γ1 ▻▻ Δ) (Γ2 ▻▻ Δ) A) : CHeapSpecM Γ1 Γ2 A :=
         fun POST δ0 => d (fun a δ1 => POST a (env.drop Δ δ1)) (δ0 ►► δΔ).
+      #[global] Arguments pushspops {_ _ _ _} δΔ d _ /.
       Definition get_local {Γ} : CHeapSpecM Γ Γ (CStore Γ) :=
         fun POST δ => POST δ δ.
+      #[global] Arguments get_local {_} _ /.
       Definition put_local {Γ1 Γ2} (δ : CStore Γ2) : CHeapSpecM Γ1 Γ2 unit :=
         fun POST _ => POST tt δ.
+      #[global] Arguments put_local {_ _} δ _ /.
 
       Definition eval_exp {Γ σ} (e : Exp Γ σ) : CHeapSpecM Γ Γ (Val σ) :=
         fun POST δ => POST (eval e δ) δ.
+      #[global] Arguments eval_exp {_ _} e _ /.
       Definition eval_exps {Γ} {σs : PCtx} (es : NamedEnv (Exp Γ) σs) : CHeapSpecM Γ Γ (CStore σs) :=
         fun POST δ => POST (evals es δ) δ.
+      #[global] Arguments eval_exps {_ _} es _ /.
       Definition assign {Γ} x {σ} {xIn : x∷σ ∈ Γ} (v : Val σ) : CHeapSpecM Γ Γ unit :=
         fun POST δ => POST tt (δ ⟪ x ↦ v ⟫).
-      Global Arguments assign {Γ} x {σ xIn} v.
+      #[global] Arguments assign {Γ} x {σ xIn} v _ /.
 
     End State.
 
-    Section ProduceConsume.
-
-      Fixpoint produce {Γ Σ} (ι : Valuation Σ) (asn : Assertion Σ) : CHeapSpecM Γ Γ unit :=
-        match asn with
-        | asn.formula fml => assume_formula (inst fml ι)
-        | asn.chunk c     => produce_chunk (inst c ι)
-        | asn.chunk_angelic c => produce_chunk (inst c ι)
-        | asn.match_bool b a1 a2  => demonic_match_bool (inst b ι) (produce ι a1) (produce ι a2)
-        | asn.match_enum E k alts =>
-          demonic_match_enum
-            (inst (T := fun Σ => Term Σ _) k ι)
-            (fun K => produce ι (alts K))
-        | asn.match_sum σ τ s xl alt_inl xr alt_inr =>
-          demonic_match_sum
-            (inst (T := fun Σ => Term Σ _) s ι)
-            (fun v => produce (env.snoc ι (xl∷σ) v) alt_inl)
-            (fun v => produce (env.snoc ι (xr∷τ) v) alt_inr)
-        | asn.match_list s alt_nil xh xt alt_cons =>
-          demonic_match_list
-            (inst (T := fun Σ => Term Σ _) s ι)
-            (produce ι alt_nil)
-            (fun vh vt => produce (ι ► (xh∷_ ↦ vh) ► (xt∷ty.list _ ↦ vt)) alt_cons)
-        | asn.match_prod s xl xr rhs =>
-          demonic_match_prod
-            (inst (T := fun Σ => Term Σ _) s ι)
-            (fun vl vr => produce (ι ► (xl∷_ ↦ vl) ► (xr∷_ ↦ vr)) rhs)
-        | asn.match_tuple s p rhs =>
-          demonic_match_tuple p
-            (inst (T := fun Σ => Term Σ _) s ι)
-            (fun ι' => produce (ι ►► ι') rhs)
-        | asn.match_record R s p rhs =>
-          demonic_match_record p
-            (inst (T := fun Σ => Term Σ _) s ι)
-            (fun ι' => produce (ι ►► ι') rhs)
-        | asn.match_union U s alt__ctx alt__pat alt__rhs =>
-          demonic_match_union
-            alt__pat (inst (T := fun Σ => Term Σ _) s ι)
-            (fun UK ι' => produce (ι ►► ι') (alt__rhs UK))
-        | asn.sep a1 a2   => _ <- produce ι a1 ;; produce ι a2
-        | asn.or a1 a2 =>
-          demonic_binary (produce ι a1)
-                         (produce ι a2)
-        | asn.exist ς τ a =>
-          v <- demonic τ ;;
-          produce (env.snoc ι (ς∷τ) v) a
-        | asn.debug => pure tt
-        end.
-
-      Fixpoint consume {Γ Σ} (ι : Valuation Σ) (asn : Assertion Σ) : CHeapSpecM Γ Γ unit :=
-        match asn with
-        | asn.formula fml => assert_formula (inst fml ι)
-        | asn.chunk c     => consume_chunk (inst c ι)
-        | asn.chunk_angelic c     => consume_chunk (inst c ι)
-        | asn.match_bool b a1 a2  => angelic_match_bool (inst b ι) (consume ι a1) (consume ι a2)
-        | asn.match_enum E k alts =>
-          angelic_match_enum
-            (inst (T := fun Σ => Term Σ _) k ι)
-            (fun K => consume ι (alts K))
-        | asn.match_sum σ τ s xl alt_inl xr alt_inr =>
-          angelic_match_sum
-            (inst (T := fun Σ => Term Σ _) s ι)
-            (fun v => consume (env.snoc ι (xl∷σ) v) alt_inl)
-            (fun v => consume (env.snoc ι (xr∷τ) v) alt_inr)
-        | asn.match_list s alt_nil xh xt alt_cons =>
-          angelic_match_list
-            (inst (T := fun Σ => Term Σ _) s ι)
-            (consume ι alt_nil)
-            (fun vh vt => consume (ι ► (xh∷_ ↦ vh) ► (xt∷ty.list _ ↦ vt)) alt_cons)
-        | asn.match_prod s xl xr rhs =>
-          angelic_match_prod
-            (inst (T := fun Σ => Term Σ _) s ι)
-            (fun vl vr => consume (ι ► (xl∷_ ↦ vl) ► (xr∷_ ↦ vr)) rhs)
-        | asn.match_tuple s p rhs =>
-          angelic_match_tuple p
-            (inst (T := fun Σ => Term Σ _) s ι)
-            (fun ι' => consume (ι ►► ι') rhs)
-        | asn.match_record R s p rhs =>
-          angelic_match_record p
-            (inst (T := fun Σ => Term Σ _) s ι)
-            (fun ι' => consume (ι ►► ι') rhs)
-        | asn.match_union U s alt__ctx alt__pat alt__rhs =>
-          angelic_match_union
-            alt__pat (inst (T := fun Σ => Term Σ _) s ι)
-            (fun UK ι' => consume (ι ►► ι') (alt__rhs UK))
-        | asn.sep a1 a2   => _ <- consume ι a1;; consume ι a2
-        | asn.or a1 a2 =>
-          angelic_binary (consume ι a1)
-                         (consume ι a2)
-        | asn.exist ς τ a =>
-          v <- angelic τ ;;
-          consume (env.snoc ι (ς∷τ) v) a
-        | asn.debug => pure tt
-        end.
-
-    End ProduceConsume.
-
     Section Exec.
-
-      Definition call_contract {Γ Δ τ} (contract : SepContract Δ τ) (args : CStore Δ) : CHeapSpecM Γ Γ (Val τ) :=
-        match contract with
-        | MkSepContract _ _ Σe δ req result ens =>
-          ι <- angelic_ctx Σe ;;
-          assert_eq_nenv (inst δ ι) args ;;
-          consume ι req  ;;
-          v <- demonic τ ;;
-          produce (env.snoc ι (result∷τ) v) ens ;;
-          pure v
-        end.
-
-      Definition call_lemma {Γ Δ} (lem : Lemma Δ) (vs : CStore Δ) : CHeapSpecM Γ Γ unit :=
-        match lem with
-        | MkLemma _ Σe δ req ens =>
-          ι <- angelic_ctx Σe ;;
-          assert_eq_nenv (inst δ ι) vs ;;
-          consume ι req ;;
-          produce ι ens
-        end.
 
       (* The paper discusses the case that a function call is replaced by
          interpreting the contract instead. However, this is not always
@@ -1046,134 +832,154 @@ Module Type ShallowExecOn
          executor in an open-recusion style and [Exec] is the closed type of
          such an executor. *)
       Definition Exec := forall Γ τ (s : Stm Γ τ), CHeapSpecM Γ Γ (Val τ).
+      Definition ExecCall := forall Δ τ, 𝑭 Δ τ -> CStore Δ -> CPureSpecM (L := L) (Val τ).
 
-      Section ExecAux.
+      Definition ExecRefine (e1 e2 : Exec) : Prop :=
+        forall Γ τ (s : Stm Γ τ) POST δ,
+          e1 _ _ s POST δ ⊢ e2 _ _ s POST δ.
+
+      Section ExecOpen.
 
         (* The executor for "inlining" a call. *)
-        Variable rec : Exec.
+        Variable exec : Exec.
+
+        Definition exec_call_inline : ExecCall :=
+          fun Δ τ f args POST =>
+            exec (FunDef f) (fun v _ => POST v) args.
+
+        Definition exec_call_with_contracts : ExecCall :=
+          fun Δ τ f args =>
+            match CEnv f with
+            | Some c => CPureSpecM.call_contract c args
+            | None   => exec_call_inline f args
+            end.
+
+        Variable exec_call : ExecCall.
 
         (* The openly-recursive executor. *)
-        Definition exec_aux : Exec :=
-          fix exec_aux {Γ τ} (s : Stm Γ τ) : CHeapSpecM Γ Γ (Val τ) :=
+        Definition exec_open : Exec :=
+          fun Γ τ s =>
             match s with
             | stm_val _ l => pure l
             | stm_exp e => eval_exp e
             | stm_let x σ s k =>
-              v <- exec_aux s ;;
-              pushpop v (exec_aux k)
+              v <- exec s ;;
+              pushpop v (exec k)
             | stm_block δ k =>
-              pushspops δ (exec_aux k)
+              pushspops δ (exec k)
             | stm_assign x e =>
-              v <- exec_aux e ;;
+              v <- exec e ;;
               _ <- assign x v ;;
               pure v
             | stm_call f es =>
               args <- eval_exps es ;;
-              match CEnv f with
-              | Some c => call_contract c args
-              | None   => fun POST δ => rec (FunDef f) (fun v _ => POST v δ) args
-              end
+              lift_purem (exec_call f args)
             | stm_foreign f es =>
               ts <- eval_exps es ;;
-              call_contract (CEnvEx f) ts
+              lift_purem (CPureSpecM.call_contract (CEnvEx f) ts)
             | stm_lemmak l es k =>
               ts <- eval_exps es ;;
-              _  <- call_lemma (LEnv l) ts ;;
-              exec_aux k
+              _  <- lift_purem (CPureSpecM.call_lemma (LEnv l) ts) ;;
+              exec k
             | stm_call_frame δ' s =>
               δ <- get_local ;;
               _ <- put_local δ' ;;
-              v <- exec_aux s ;;
+              v <- exec s ;;
               _ <- put_local δ ;;
               pure v
             | stm_if e s1 s2 =>
               v <- eval_exp e ;;
-              demonic_match_bool v (exec_aux s1) (exec_aux s2)
-            | stm_seq e k => _ <- exec_aux e ;; exec_aux k
+              match_bool v (exec s1) (exec s2)
+            | stm_seq e k => _ <- exec e ;; exec k
             | stm_assertk e1 _ k =>
               v <- eval_exp e1 ;;
-              _ <- assume_formula (v = true) ;;
-              exec_aux k
+              _ <- lift_purem (CPureSpecM.assume_formula (v = true)) ;;
+              exec k
             | stm_fail _ s =>
               block
             | stm_match_enum E e alts =>
               v <- eval_exp e ;;
-              demonic_match_enum
+              match_enum
                 v
-                (fun EK => exec_aux (alts EK))
+                (fun EK => exec (alts EK))
             | stm_read_register reg =>
               v <- angelic τ ;;
               let c := scchunk_ptsreg reg v in
-              _ <- consume_chunk c ;;
-              _ <- produce_chunk c ;;
+              _ <- lift_purem (CPureSpecM.consume_chunk c) ;;
+              _ <- lift_purem (CPureSpecM.produce_chunk c) ;;
               pure v
             | stm_write_register reg e =>
               v__old <- angelic τ ;;
-              _    <- consume_chunk (scchunk_ptsreg reg v__old) ;;
+              _    <- lift_purem (CPureSpecM.consume_chunk (scchunk_ptsreg reg v__old)) ;;
               v__new <- eval_exp e ;;
-              _    <- produce_chunk (scchunk_ptsreg reg v__new) ;;
+              _    <- lift_purem (CPureSpecM.produce_chunk (scchunk_ptsreg reg v__new)) ;;
               pure v__new
             | @stm_match_list _ _ σ e s1 xh xt s2 =>
               v <- eval_exp e ;;
-              demonic_match_list v
-                (exec_aux s1)
+              match_list v
+                (exec s1)
                 (fun h t =>
                    pushspops
                      (env.snoc (env.snoc env.nil (xh∷σ) h) (xt∷ty.list σ) t)
-                     (exec_aux s2))
+                     (exec s2))
             | stm_match_sum e xinl s1 xinr s2 =>
               v <- eval_exp e ;;
-              demonic_match_sum
+              match_sum
                 v
-                (fun v => pushpop v (exec_aux s1))
-                (fun v => pushpop v (exec_aux s2))
-            | stm_match_prod e xl xr s =>
+                (fun v => pushpop v (exec s1))
+                (fun v => pushpop v (exec s2))
+            | stm_match_prod e xl xr rhs =>
               v <- eval_exp e ;;
-              demonic_match_prod
-                v
+              match_prod v
                 (fun vl vr =>
-                   pushspops
-                     (env.snoc (env.snoc env.nil (xl∷_) vl) (xr∷_) vr)
-                     (exec_aux s))
+                   pushspops [kv (xl∷_; vl); (xr∷_; vr)] (exec rhs))
             | stm_match_tuple e p rhs =>
               v <- eval_exp e ;;
-              demonic_match_tuple p v
-                (fun δΔ => pushspops δΔ (exec_aux rhs))
+              match_tuple p v
+                (fun δΔ => pushspops δΔ (exec rhs))
             | stm_match_union U e alt__pat alt__rhs =>
               v <- eval_exp e ;;
-              demonic_match_union alt__pat v (fun UK vs => pushspops vs (exec_aux (alt__rhs UK)))
+              match_union alt__pat v (fun UK vs => pushspops vs (exec (alt__rhs UK)))
             | stm_match_record R e p rhs =>
               v <- eval_exp e ;;
-              demonic_match_record p v (fun vs => pushspops vs (exec_aux rhs))
+              match_record p v (fun vs => pushspops vs (exec rhs))
             | stm_match_bvec n e rhs =>
               v <- eval_exp e ;;
-              demonic_match_bvec
+              match_bvec
                 v
-                (fun u => exec_aux (rhs u))
+                (fun u => exec (rhs u))
             | stm_match_bvec_split m n e xl xr rhs =>
               v <- eval_exp e ;;
-              demonic_match_bvec_split
+              match_bvec_split
                 v
                 (fun vl vr =>
                    pushspops
                      [kv (xl∷ty.bvec m; vl); (xr∷ty.bvec n; vr)]
-                     (exec_aux rhs))
+                     (exec rhs))
             | stm_bind s k =>
-              v <- exec_aux s ;;
-              exec_aux (k v)
+              v <- exec s ;;
+              exec (k v)
             | stm_debugk k =>
-              exec_aux k
+              exec k
             end.
 
-      End ExecAux.
+      End ExecOpen.
+      #[global] Arguments exec_call_with_contracts exec [_ _] f args _ /.
+
+      Definition exec_error : Exec :=
+        fun _ _ _ => error.
+      Definition exec_def (rec : Exec) : Exec :=
+        exec_open rec (exec_call_inline rec).
+      Definition exec_aux (exec_call : ExecCall) : Exec :=
+        fix exec_aux Γ τ s := exec_open exec_aux exec_call s.
 
       (* The constructed closed executor. *)
       Fixpoint exec (inline_fuel : nat) : Exec :=
         match inline_fuel with
-        | O   => fun _ _ _ => error
-        | S n => @exec_aux (@exec n)
+        | O   => exec_error
+        | S n => exec_aux (exec_call_with_contracts (exec n))
         end.
-      Global Arguments exec _ [_ _] s _ _.
+      #[global] Arguments exec _ [_ _] s _ _.
 
     End Exec.
 
@@ -1186,9 +992,9 @@ Module Type ShallowExecOn
         match c with
         | MkSepContract _ _ _ _ req result ens =>
           fun ι =>
-          _ <- produce ι req ;;
+          _ <- lift_purem (CPureSpecM.produce ι req) ;;
           v <- exec inline_fuel s ;;
-          consume (env.snoc ι (result∷τ) v) ens
+          lift_purem (CPureSpecM.consume (env.snoc ι (result∷τ) v) ens)
         end%mut.
 
       Definition vcgen {Δ τ} (c : SepContract Δ τ) (body : Stm Δ τ) : Prop :=
@@ -1198,16 +1004,300 @@ Module Type ShallowExecOn
              nodes in a shallowly-generated VC. *)
           ⊤ ⊢ exec_contract c body ι (fun _ _ => ⊤) δΔ).
 
+      Definition vcgen' {Δ τ} (c : SepContract Δ τ) (body : Stm Δ τ) : Prop :=
+        match c with
+        | MkSepContract _ _ Σ δ req result ens =>
+            forall ι : Valuation Σ,
+              asn.interpret req ι ⊢
+              exec inline_fuel body
+                (fun v _ => asn.interpret ens (env.snoc ι (result∷τ) v)) (inst δ ι)
+        end.
+
     End WithFuel.
+
+    (* This section verifies the monotonicity of the calculated predicate
+       transformers. Which is a necessity for the main soundness theorems. *)
+    Section Monotonicity.
+
+      Import sep.instances.
+
+      #[local] Open Scope signature.
+
+      Definition Monotonic {Γ1 Γ2 A} : relation (CHeapSpecM Γ1 Γ2 A) :=
+        (A ::> CStore Γ2 ::> lentails) ==> CStore Γ1 ::> lentails.
+      Definition Monotonic' {Γ1 Γ2 A} : relation (CHeapSpecM Γ1 Γ2 A) :=
+        (A -> CStore Γ2 -> L) ::> CStore Γ1 ::> lentails.
+
+      Definition MonotonicExec : relation Exec :=
+        ∀ Γ τ, Stm Γ τ ::> Monotonic.
+      Definition MonotonicExec' : relation Exec :=
+        ∀ Γ τ, Stm Γ τ ::> Monotonic'.
+      Definition MonotonicCall : relation ExecCall :=
+        ∀ Δ σ, 𝑭 Δ σ ::> CStore Δ ::> CPureSpecM.Monotonic.
+
+      #[export] Instance monotonic_transitive {Γ1 Γ2 A} :
+        Transitive (@Monotonic Γ1 Γ2 A).
+      Proof.
+        intros f g h fg gh P Q PQ δ. transitivity (g Q δ).
+        apply fg. assumption. apply gh. reflexivity.
+      Qed.
+
+      #[export] Instance monotonicexec_transitive :
+        Transitive MonotonicExec.
+      Proof.
+        intros f g h fg gh Γ τ s.
+        transitivity (g Γ τ s); [apply fg|apply gh].
+      Qed.
+
+      Ltac solve_monotonic :=
+        repeat
+          lazymatch goal with
+          | |- ?x           ⊢ ?x => reflexivity
+          | |- Basics.flip lentails ?x ?y => change_no_check (lentails y x)
+          | |- limpl _ _    ⊢ _  => apply proper_limpl_entails; [easy|]
+          | |- lsep _ _     ⊢ _  => apply proper_lsep_entails
+          | |- lwand _ _    ⊢ _  => apply proper_lwand_entails
+          | |- lex _        ⊢ _  => apply proper_lex_entails; intros ?
+          | H : (_ ::> CStore _ ::> lentails) ?P ?Q |- ?P ?x ?δ ⊢ ?Q ?x ?δ =>
+              apply H
+          | H : Monotonic ?m1 ?m2 |- ?m1 _ ?δ ⊢ ?m2 _ ?δ =>
+              apply H; intros ? ?
+          | H: MonotonicExec ?ex1 ?ex2 |- ?ex1 _ _ ?s _ _ ⊢ ?ex2 _ _ ?s _ _ =>
+              apply H; intros ? ?
+          | H: MonotonicCall ?ec1 ?ec2 |- ?ec1 _ _ ?f _ _ ⊢ ?ec2 _ _ ?f _ _ =>
+              apply H; intros ?
+          | H: Proper MonotonicCall ?ec |- ?ec _ _ ?f _ _ ⊢ ?ec _ _ ?f _ _ =>
+              apply H; intros ?
+          (* | H: forall _, Monotonic (?f _) (?g _) |- ?f _ _ ?δ ⊢ ?g _ _ ?δ => *)
+          (*     apply H; intros ? ? *)
+          | H: forall _, Monotonic (?f _ _ _) (?g _ _ _) |- ?f _ _ _ _ _ ⊢ ?g _ _ _ _ _ =>
+              apply H; intros ? ?
+          | |- CPureSpecM.call_contract _ _ _ ⊢ _ =>
+              apply CPureSpecM.monotonic_call_contract; intros ?
+          | |- CPureSpecM.call_lemma _ _ _ ⊢ _ =>
+              apply CPureSpecM.monotonic_call_lemma; intros ?
+          | |- (match ?x with _ => _ end) ⊢ _ => destruct x
+          | |- Proper _ _ => unfold Proper
+          | |- Monotonic _ _ => intros ?P ?Q ?PQ ?δ; cbn
+          | |- respectful _ _ _ _ => intros ? ? ?
+          | H: (_ ::> Monotonic) ?f ?g |- ?f _ _ _ ⊢ ?g _ _ _ =>
+              apply H; intros ? ?
+          end.
+
+      Instance exec_call_inline_monotonic :
+        Proper (MonotonicExec ==> MonotonicCall) (exec_call_inline).
+      Proof. intros ex1 ex2 ex_mon Δ σ f args P Q PQ. now apply ex_mon. Qed.
+
+      Instance exec_call_with_contracts_monotonic :
+        Proper (MonotonicExec ==> MonotonicCall) (exec_call_with_contracts).
+      Proof.
+        intros ex1 ex2 ex_mon Δ σ f args.
+        unfold exec_call_with_contracts. destruct CEnv.
+        - apply CPureSpecM.monotonic_call_contract.
+        - now apply exec_call_inline_monotonic.
+      Qed.
+
+      Instance exec_open_monotonic :
+        Proper (MonotonicExec ==> MonotonicCall ==> MonotonicExec) exec_open.
+      Proof.
+        intros ex1 ex2 ex_mon ec1 ec2 ec_mon Γ τ s P Q PQ δΓ.
+        destruct s; cbn; solve_monotonic.
+      Qed.
+
+      Instance exec_def_monotonic :
+        Proper (MonotonicExec ==> MonotonicExec) exec_def.
+      Proof.
+        intros ex1 ex2 ex_mon. unfold exec_def.
+        now apply exec_open_monotonic, exec_call_inline_monotonic.
+      Qed.
+
+      Instance exec_aux_monotonic :
+        Proper (MonotonicCall ==> MonotonicExec) (exec_aux).
+      Proof.
+        intros ec1 ec2 ec_mon Γ τ s.
+        induction s; intros P Q PQ ?; cbn; solve_monotonic.
+      Qed.
+
+      Lemma fold_exec_aux (ex : Exec) (ec : ExecCall)
+        (IHc : Proper MonotonicCall ec)
+        (IHx : MonotonicExec (exec_open ex ec) ex) :
+        MonotonicExec (exec_aux ec) ex.
+      Proof.
+        intros Γ τ s; induction s; cbn [exec_aux];
+          match goal with
+          | |- Monotonic (exec_open _ _ ?s) (ex _ _ ?s) =>
+              transitivity (exec_open ex ec s);
+              [cbn [exec_open]|apply IHx]
+          end;
+          solve_monotonic.
+      Qed.
+
+      Lemma exec_error_initial (ex : Exec) :
+        MonotonicExec exec_error ex.
+      Proof. intros ? ? ? ? ? ? ?. apply lfalse_left. Qed.
+
+      Lemma exec_monotonic n : Proper MonotonicExec (exec n).
+      Proof.
+        induction n; cbn.
+        - apply exec_error_initial.
+        - now apply exec_aux_monotonic, exec_call_with_contracts_monotonic.
+      Qed.
+
+      Record Model (ex : Exec) : Prop := {
+          rule_syntactic :
+            MonotonicExec'
+              (exec_def ex)
+              ex;
+
+          rule_contract :
+            MonotonicCall
+              (exec_call_with_contracts exec_error)
+              (exec_call_inline ex);
+
+          ex_monotonic :> Proper MonotonicExec ex;
+        }.
+
+    End Monotonicity.
+
+    Import sep.instances.
+
+    Lemma vcgen_equiv {Δ τ} n (c : SepContract Δ τ) (body : Stm Δ τ) :
+      vcgen n c body <-> vcgen' n c body.
+    Proof.
+      destruct c as [Σ δ req result ens]; cbn.
+      rewrite env.Forall_forall.
+      apply base.forall_proper; intros ι.
+      rewrite CPureSpecM.wp_produce.
+      rewrite <- lwand_sep_adjoint.
+      apply proper_entails_equiv_iff.
+      rewrite lsep_true. reflexivity.
+      split; apply exec_monotonic; intros v δ';
+        now rewrite CPureSpecM.wp_consume, lsep_comm, lsep_true.
+    Qed.
+
   End WithProp.
   End CHeapSpecM.
   Export CHeapSpecM (CHeapSpecM).
 
+
   Module Shallow.
 
-    Definition ValidContract L {PI : PredicateDef L} {Δ τ} (c : SepContract Δ τ) (body : Stm Δ τ) : Prop :=
-      (* Use inline_fuel = 1 by default. *)
-      CHeapSpecM.vcgen (L := L) 1 c body.
+    Import sep.instances.
+
+    Section Soundness.
+      Context {L} {PI : PredicateDef L}.
+
+      Definition ValidContract {Δ τ} (c : SepContract Δ τ) (body : Stm Δ τ) : Prop :=
+        (* Use inline_fuel = 1 by default. *)
+        CHeapSpecM.vcgen (L := L) 1 c body.
+
+      Definition ValidContractCEnv : Prop :=
+        forall (Δ : PCtx) (τ : Ty) (f : 𝑭 Δ τ) (c : SepContract Δ τ),
+          CEnv f = Some c ->
+          ValidContract c (FunDef f).
+
+      Import CHeapSpecM.
+
+      Lemma rule_syntactic' (ec : ExecCall) (ec_mon : Proper MonotonicCall ec)
+        (ex : Exec) (ex_mdl : Model ex) :
+        MonotonicCall ec (exec_call_inline ex) ->
+        MonotonicExec (exec_aux ec) ex.
+      Proof.
+        intros. apply fold_exec_aux; [assumption|].
+        transitivity (exec_open ex (exec_call_inline ex)).
+        apply exec_open_monotonic.
+        apply ex_monotonic; auto.
+        assumption.
+        intros Γ τ s P Q PQ δ.
+        transitivity (ex _ _ s P δ).
+        apply (rule_syntactic ex_mdl).
+        apply ex_monotonic; auto.
+      Qed.
+
+      Definition ValidContractSem (ex : Exec) {Δ σ} (body : Stm Δ σ) (contract : SepContract Δ σ) : L :=
+        match contract with
+        | MkSepContract _ _ ctxΣ θΔ req res ens =>
+            ∀ (ι : Valuation ctxΣ),
+              asn.interpret req ι -∗
+               ex _ _ body (fun v _ => asn.interpret ens ι.[res∷σ ↦ v]) (inst θΔ ι)
+        end.
+
+      Definition ValidContractEnvSem (ex : Exec) : L :=
+        ∀ Δ σ (f : 𝑭 Δ σ),
+          match CEnv f with
+          | Some c => ValidContractSem ex (FunDef f) c
+          | None   => ⊤
+          end.
+
+      Lemma validcontractsem_monotonic :
+        Proper
+          (MonotonicExec ==> ∀ Γ τ, Stm Γ τ ::> SepContract Γ τ ::> lentails)
+          ValidContractSem.
+      Proof.
+        intros ex1 ex2 ex_mon Γ τ s [Σe δΔ req res ens]; cbn.
+        apply proper_lall_entails; intros ι.
+        apply proper_lwand_entails; [easy|].
+        now apply ex_mon.
+      Qed.
+
+      Instance validcontractenvsem_monotonic :
+        Proper (MonotonicExec ==> lentails) ValidContractEnvSem.
+      Proof.
+        intros ex1 ex2 ex_mon.
+        unfold ValidContractEnvSem.
+        apply proper_lall_entails; intros Δ.
+        apply proper_lall_entails; intros σ.
+        apply proper_lall_entails; intros f.
+        destruct CEnv; [|easy].
+        now apply validcontractsem_monotonic.
+      Qed.
+
+      Definition sound_shallow (vcenv : ValidContractCEnv) :
+        ⊤ ⊢ ValidContractEnvSem (exec 1).
+      Proof.
+        apply lall_right; intros Δ.
+        apply lall_right; intros σ.
+        apply lall_right; intros f.
+        specialize (vcenv Δ σ f).
+        destruct (CEnv f) as [ctr|]; [|easy].
+        specialize (vcenv _ eq_refl).
+        unfold ValidContract in vcenv.
+        rewrite vcgen_equiv in vcenv.
+        destruct ctr as [Σe δΔ req res ens].
+        apply lall_right; intros ι.
+        specialize (vcenv ι).
+        apply lwand_sep_adjoint.
+        now rewrite lsep_true.
+      Qed.
+
+      Lemma soundness (ex : Exec) (exmdl : Model ex) :
+        ValidContractCEnv -> ⊤ ⊢ ValidContractEnvSem ex.
+      Proof.
+        unfold ValidContractCEnv.
+        intros vcenv.
+        apply lall_right; intros Δ.
+        apply lall_right; intros σ.
+        apply lall_right; intros f.
+        specialize (vcenv Δ σ f).
+        destruct (CEnv f) as [ctr|]; [|easy].
+        specialize (vcenv ctr eq_refl).
+        destruct ctr as [ctxΣ θΔ req res ens]; cbn in *.
+        apply lall_right; intros ι.
+        rewrite env.Forall_forall in vcenv.
+        specialize (vcenv ι). revert vcenv.
+        apply proper_entails_entails_impl; [easy|].
+        rewrite CPureSpecM.wp_produce.
+        apply proper_lwand_entails; [easy|].
+        apply rule_syntactic'; auto.
+        apply exec_call_with_contracts_monotonic.
+        apply exec_error_initial.
+        apply rule_contract; auto.
+        intros ? ?.
+        rewrite CPureSpecM.wp_consume.
+        now rewrite lsep_comm, lsep_true.
+      Qed.
+
+    End Soundness.
 
     Module Statistics.
 
@@ -1328,14 +1418,14 @@ Module Type ShallowExecOn
 
   End Shallow.
 
-End ShallowExecOn.
+End NewShallowExecOn.
 
-Module MakeShallowExecutor
+Module MakeNewShallowExecutor
   (Import B    : Base)
   (Import PROG : Program B)
   (Import SIG : Signature B)
   (Import SPEC : Specification B PROG SIG).
 
-  Include ShallowExecOn B PROG SIG SPEC.
+  Include NewShallowExecOn B PROG SIG SPEC.
 
-End MakeShallowExecutor.
+End MakeNewShallowExecutor.
