theories/Staging/NewShallow/Soundness.v
@@ -49,7 +49,7 @@ Module Type Soundness
   (Import PROG : Program B)
   (Import SIG : Signature B)
   (Import SPEC : Specification B PROG SIG)
-  (Import EXEC : ShallowExecOn B PROG SIG SPEC)
+  (Import EXEC : NewShallowExecOn B PROG SIG SPEC)
   (Import HOAR : ProgramLogicOn B PROG SIG SPEC).
 
   Import sep.instances.
@@ -61,295 +61,31 @@ Module Type Soundness
 
     Context {L} {PI : PredicateDef L}.
 
-    (* This section verifies the monotonicity of the calculated predicate
-       transformers. Which is a necessity for the main soundness theorems. *)
-    Section Monotonicity.
-
-      Definition Monotonic {Γ1 Γ2 A} (m : CHeapSpecM Γ1 Γ2 A) : Prop :=
-        forall
-          (P Q : A -> CStore Γ2 -> L)
-          (PQ : forall x δ, P x δ ⊢ Q x δ),
-          forall δ, m P δ ⊢ m Q δ.
-
-      (* Stronger version for those that do not change the store. *)
-      Definition Monotonic' {Γ A} (m : CHeapSpecM Γ Γ A) : Prop :=
-        forall δ
-          (P Q : A -> CStore Γ -> L)
-          (PQ : forall x, P x δ ⊢ Q x δ),
-          m P δ ⊢ m Q δ.
-
-      Lemma consume_chunk_monotonic {Γ} {c : SCChunk} :
-        Monotonic' (consume_chunk (Γ := Γ) c).
-      Proof. intros δ P Q PQ. now apply proper_lsep_entails. Qed.
-
-      Lemma produce_chunk_monotonic {Γ} {c : SCChunk} :
-        Monotonic' (produce_chunk (Γ := Γ) c).
-      Proof. intros δ P Q PQ. now apply proper_lwand_entails. Qed.
-
-      Lemma consume_monotonic {Γ Σ} {ι : Valuation Σ} {asn : Assertion Σ} :
-        Monotonic' (consume (Γ := Γ) ι asn).
-      Proof.
-        intros δ. induction asn; cbn; intros * PQ *.
-        - now apply proper_land_entails.
-        - now apply consume_chunk_monotonic.
-        - now apply consume_chunk_monotonic.
-        - rewrite ?wp_angelic_match_bool. destruct (inst b ι); cbn; auto.
-        - rewrite ?wp_angelic_match_enum; auto.
-        - rewrite ?wp_angelic_match_sum. destruct (inst s ι); cbn; auto.
-        - rewrite ?wp_angelic_match_list. destruct (inst s ι); cbn; auto.
-        - rewrite ?wp_angelic_match_prod. destruct (inst s ι); cbn; auto.
-        - rewrite ?wp_angelic_match_tuple; auto.
-        - rewrite ?wp_angelic_match_record; auto.
-        - rewrite ?wp_angelic_match_union. destruct (unionv_unfold U (inst s ι)); auto.
-        - unfold bind; auto.
-        - apply proper_lor_entails; auto.
-        - apply proper_lex_entails; intros v; auto.
-        - unfold pure; auto.
-      Qed.
-
-      Lemma produce_monotonic {Γ Σ} {ι : Valuation Σ} {asn : Assertion Σ} :
-        Monotonic' (produce (Γ := Γ) ι asn).
-      Proof.
-        intros δ. induction asn; cbn; intros * PQ *.
-        - now apply proper_limpl_entails.
-        - now apply produce_chunk_monotonic.
-        - now apply produce_chunk_monotonic.
-        - rewrite ?wp_demonic_match_bool. destruct (inst b ι); cbn; eauto.
-        - rewrite ?wp_demonic_match_enum; eauto.
-        - rewrite ?wp_demonic_match_sum. destruct (inst s ι); cbn; eauto.
-        - rewrite ?wp_demonic_match_list. destruct (inst s ι); cbn; eauto.
-        - rewrite ?wp_demonic_match_prod. destruct (inst s ι); cbn; eauto.
-        - rewrite ?wp_demonic_match_tuple; eauto.
-        - rewrite ?wp_demonic_match_record; eauto.
-        - rewrite ?wp_demonic_match_union. destruct (unionv_unfold U (inst s ι)); eauto.
-        - unfold bind; auto.
-        - apply proper_land_entails; auto.
-        - apply proper_lall_entails; intros v; auto.
-        - unfold pure; eauto.
-      Qed.
-
-      Lemma call_lemma_monotonic {Γ Δ} (lem : Lemma Δ) (δΔ : CStore Δ) :
-        Monotonic (call_lemma (Γ := Γ) lem δΔ).
-      Proof.
-        destruct lem; intros P Q PQ δ;
-          cbv [call_lemma bind bind_right
-               angelic_ctx lift_purem assert_formula
-               CPureSpecM.assert_formula].
-        rewrite ?CPureSpecM.wp_angelic_ctx.
-        apply proper_lex_entails; intros ι.
-        unfold assert_eq_nenv, lift_purem.
-        rewrite ?CPureSpecM.wp_assert_eq_nenv.
-        apply proper_land_entails; [easy|].
-        apply consume_monotonic. intros _.
-        apply produce_monotonic; auto.
-      Qed.
-
-      Lemma call_contract_monotonic {Γ Δ τ} (c : SepContract Δ τ) (δΔ : CStore Δ) :
-        Monotonic (call_contract (Γ := Γ) c δΔ).
-      Proof.
-        destruct c; intros P Q PQ δ;
-          cbv [call_contract bind_right bind pure demonic
-               angelic_ctx demonic lift_purem assert_formula
-               CPureSpecM.assert_formula].
-        rewrite ?CPureSpecM.wp_angelic_ctx.
-        apply proper_lex_entails; intros ι.
-        unfold assert_eq_nenv, lift_purem.
-        rewrite ?CPureSpecM.wp_assert_eq_nenv.
-        apply proper_land_entails; [easy|].
-        apply consume_monotonic. intros _.
-        apply proper_lall_entails; intros v.
-        apply produce_monotonic; auto.
-      Qed.
-
-      Definition MonotonicExec (ex : Exec) : Prop :=
-        forall Γ τ (s : Stm Γ τ),
-          Monotonic (ex _ _ s).
-
-      Lemma exec_aux_monotonic rec (rec_mono : MonotonicExec rec) :
-        MonotonicExec (exec_aux rec).
-      Proof.
-        unfold MonotonicExec. intros ? ? s.
-        induction s; cbn; intros P Q PQ *;
-          cbv [pure bind angelic pushpop pushspops
-               put_local get_local eval_exp eval_exps assign].
-        - auto.
-        - auto.
-        - apply IHs1. intros *. apply IHs2. auto.
-        - apply IHs. auto.
-        - apply IHs. auto.
-        - destruct (CEnv f); cbn; auto.
-          + apply call_contract_monotonic; auto.
-          + apply rec_mono; auto.
-        - apply IHs. auto.
-        - apply call_contract_monotonic; auto.
-        - apply call_lemma_monotonic; intros ? ?.
-          apply IHs. auto.
-        - rewrite ?wp_demonic_match_bool.
-          destruct (eval e δ); [apply IHs1|apply IHs2]; auto.
-        - apply IHs1. intros ? ?. apply IHs2. auto.
-        - apply proper_limpl_entails; [easy|]. now apply IHs.
-        - easy.
-        - rewrite ?wp_demonic_match_list.
-          destruct (eval e δ); [apply IHs1|apply IHs2]; auto.
-        - rewrite ?wp_demonic_match_sum.
-          destruct (eval e δ); [apply IHs1|apply IHs2]; auto.
-        - rewrite ?wp_demonic_match_prod.
-          destruct (eval e δ); apply IHs; auto.
-        - rewrite ?wp_demonic_match_enum.
-          apply H; auto.
-        - rewrite ?wp_demonic_match_tuple.
-          apply IHs; auto.
-        - rewrite ?wp_demonic_match_union.
-          destruct (unionv_unfold U (eval e δ)).
-          apply H; auto.
-        - rewrite ?wp_demonic_match_record.
-          apply IHs; auto.
-        - rewrite ?wp_demonic_match_bvec.
-          apply H; auto.
-        - rewrite ?wp_demonic_match_bvec_split.
-          destruct bv.appView. apply IHs; auto.
-        - apply proper_lex_entails; intros v.
-          apply consume_chunk_monotonic. intros _.
-          now apply produce_chunk_monotonic.
-        - apply proper_lex_entails; intros v.
-          apply consume_chunk_monotonic. intros _.
-          now apply produce_chunk_monotonic.
-        - apply IHs; intros *; apply H; auto.
-        - apply IHs; auto.
-      Qed.
-
-      Lemma exec_monotonic n : MonotonicExec (exec n).
-      Proof.
-        induction n; cbn.
-        - unfold MonotonicExec, Monotonic, error; easy.
-        - now apply exec_aux_monotonic.
-      Qed.
-
-    End Monotonicity.
-
-    Lemma scchunk_duplicate (c : SCChunk) :
-      is_duplicable c = true -> interpret_scchunk c ⊢@{L} interpret_scchunk c ∗ interpret_scchunk c.
-    Proof.
-      destruct c; cbn; try discriminate.
-      eauto using lduplicate.
-    Qed.
-
-    Lemma assert_formula_sound {Γ Σ} {ι : Valuation Σ} {fml : Formula Σ} (POST : unit -> CStore Γ -> L) δ :
-      assert_formula (inst fml ι) POST δ ⊣⊢ (!! inst fml ι ∧ lemp) ∗ POST tt δ.
-    Proof. now rewrite lemp_true, land_true, lprop_sep_and. Qed.
-
-    Lemma assume_formula_sound {Γ Σ} {ι : Valuation Σ} {fml : Formula Σ} (POST : unit -> CStore Γ -> L) δ :
-      assume_formula (inst fml ι) POST δ ⊣⊢ ((!! inst fml ι ∧ lemp) -∗ POST tt δ).
-    Proof. now rewrite lemp_true, land_true, lprop_wand_impl. Qed.
-
-    Lemma interpret_scchunk_inst {Σ} (c : Chunk Σ) (ι : Valuation Σ) :
-      interpret_scchunk (inst c ι) = interpret_chunk c ι.
-    Proof.
-      induction c; cbn [interpret_chunk];
-        try rewrite <- IHc1, <- IHc2; reflexivity.
-    Qed.
-
-    Lemma consume_sound {Γ Σ} {ι : Valuation Σ} {asn : Assertion Σ} (POST : unit -> CStore Γ -> L) :
-      forall δ,
-        consume ι asn POST δ ⊣⊢ asn.interpret asn ι ∗ POST tt δ.
-    Proof.
-      revert POST. induction asn; cbn - [inst inst_term]; intros POST δ1.
-      - apply assert_formula_sound.
-      - unfold consume_chunk; now rewrite interpret_scchunk_inst.
-      - unfold consume_chunk; now rewrite interpret_scchunk_inst.
-      - rewrite wp_angelic_match_bool.
-        destruct (inst b ι); auto.
-      - rewrite wp_angelic_match_enum; auto.
-      - rewrite wp_angelic_match_sum.
-        destruct (inst s ι); auto.
-      - rewrite wp_angelic_match_list.
-        destruct (inst s ι); auto.
-      - rewrite wp_angelic_match_prod.
-        destruct (inst s ι); auto.
-      - rewrite wp_angelic_match_tuple; auto.
-      - rewrite wp_angelic_match_record; auto.
-      - rewrite wp_angelic_match_union.
-        destruct (unionv_unfold U (inst s ι)); auto.
-      - unfold bind. now rewrite IHasn1, IHasn2, <- lsep_assoc.
-      - rewrite lsep_disj_distr. now apply proper_lor_equiv.
-      - rewrite lsep_exists_comm. now apply proper_lex_equiv.
-      - now rewrite lsep_comm, lsep_emp.
-    Qed.
-
-    Lemma produce_sound {Γ Σ} {ι : Valuation Σ} {asn : Assertion Σ} (POST : unit -> CStore Γ -> L) :
-      forall δ,
-        produce ι asn POST δ ⊣⊢ (asn.interpret asn ι -∗ POST tt δ).
-    Proof.
-      revert POST. induction asn; cbn - [inst inst_term]; intros POST δ1.
-      - apply assume_formula_sound.
-      - unfold produce_chunk; now rewrite interpret_scchunk_inst.
-      - unfold produce_chunk; now rewrite interpret_scchunk_inst.
-      - rewrite wp_demonic_match_bool.
-        destruct (inst b ι); auto.
-      - rewrite wp_demonic_match_enum; auto.
-      - rewrite wp_demonic_match_sum.
-        destruct (inst s ι); auto.
-      - rewrite wp_demonic_match_list.
-        destruct (inst s ι); auto.
-      - rewrite wp_demonic_match_prod.
-        destruct (inst s ι); auto.
-      - rewrite wp_demonic_match_tuple; auto.
-      - rewrite wp_demonic_match_record; auto.
-      - rewrite wp_demonic_match_union.
-        destruct (unionv_unfold U (inst s ι)); auto.
-      - unfold bind. now rewrite IHasn1, IHasn2, lwand_curry.
-      - unfold demonic_binary. now rewrite IHasn1, IHasn2, lwand_disj_distr.
-      - unfold bind, demonic. rewrite lwand_exists_comm.
-        now apply proper_lall_equiv.
-      - now rewrite lwand_emp.
-    Qed.
-
-    Lemma call_contract_sound {Γ Δ τ} (δΓ : CStore Γ)
-      (c : SepContract Δ τ) (δΔ : CStore Δ) (POST : Val τ -> CStore Γ -> L) :
-      CTriple δΔ (call_contract c δΔ POST δΓ) (fun v => POST v δΓ) c.
+    Lemma call_contract_sound {Δ τ}
+      (c : SepContract Δ τ) (δΔ : CStore Δ) (POST : Val τ -> L) :
+      CTriple δΔ (CPureSpecM.call_contract c δΔ POST) POST c.
     Proof.
       destruct c as [Σe δe req result ens]. constructor.
-      cbv [call_contract bind_right bind pure
-           angelic_ctx assert_eq_nenv lift_purem demonic].
-      rewrite CPureSpecM.wp_angelic_ctx.
-      apply proper_lex_entails. intros ι.
-      rewrite CPureSpecM.wp_assert_eq_nenv.
-      apply proper_land_entails.
-      now apply proper_lprop_entails.
-      rewrite consume_sound.
-      apply proper_lsep_entails; [easy|].
-      apply proper_lall_entails. intros v.
-      now apply produce_sound.
+      now rewrite CPureSpecM.equiv_call_contract.
     Qed.
 
-    Lemma call_lemma_sound {Γ Δ} (δΓ : CStore Γ)
-      (lem : Lemma Δ) (δΔ : CStore Δ) (POST : unit -> CStore Γ -> L) :
-      LTriple δΔ (call_lemma lem δΔ POST δΓ) (POST tt δΓ) lem.
+    Lemma call_lemma_sound {Δ}
+      (lem : Lemma Δ) (δΔ : CStore Δ) (POST : unit -> L) :
+      LTriple δΔ (CPureSpecM.call_lemma lem δΔ POST) (POST tt) lem.
     Proof.
       destruct lem as [Σe δe req ens]. constructor.
-      cbv [call_lemma bind_right bind angelic_ctx assert_eq_nenv lift_purem].
-      rewrite CPureSpecM.wp_angelic_ctx.
-      apply proper_lex_entails. intros ι.
-      rewrite CPureSpecM.wp_assert_eq_nenv.
-      apply proper_land_entails.
-      now apply proper_lprop_entails.
-      rewrite consume_sound.
-      apply proper_lsep_entails; [easy|].
-      now apply produce_sound.
+      now rewrite CPureSpecM.equiv_call_lemma.
     Qed.
 
-    Definition SoundExec (rec : Exec) :=
+    Definition SoundExec (rec : Exec) : Prop :=
       forall Γ σ (s : Stm Γ σ) (POST : Val σ -> CStore Γ -> L) (δ1 : CStore Γ),
         ⦃ rec _ _ s POST δ1 ⦄ s ; δ1 ⦃ POST ⦄.
 
-    Lemma exec_aux_sound rec (rec_mono : MonotonicExec rec) (rec_sound : SoundExec rec) :
-      SoundExec (exec_aux rec).
+    Lemma exec_aux_sound rec (rec_sound : SoundExec rec) :
+      SoundExec (exec_aux (exec_call_with_contracts rec)).
     Proof.
       unfold SoundExec. intros ? ? s.
-      induction s; intros ? ?; cbn;
-        cbv [pure pushspops pushpop
-             eval_exp get_local put_local
-             bind].
+      induction s; intros ? ?; cbn.
 
       - (* stm_val *)
         now apply rule_stm_val.
@@ -393,7 +129,6 @@ Module Type Soundness
         apply IHs.
 
       - (* stm_if *)
-        rewrite wp_demonic_match_bool.
         apply rule_stm_if; apply rule_pull; intro Heval; rewrite Heval in *; auto.
 
       - (* stm_seq *)
@@ -403,7 +138,6 @@ Module Type Soundness
         apply rule_stm_assert, rule_pull;
           intro Heval; rewrite Heval.
         eapply rule_consequence_left. apply IHs.
-        unfold assume_formula, lift_purem, CPureSpecM.assume_formula.
         now apply lentails_apply, lprop_right.
 
       - (* stm_fail *)
@@ -412,49 +146,40 @@ Module Type Soundness
         apply ltrue_right.
 
       - (* stm_match_list *)
-        rewrite wp_demonic_match_list.
         apply rule_stm_match_list; cbn; intros;
           apply rule_pull; intro Heval; rewrite Heval.
         + now apply IHs1.
         + now apply IHs2.
 
       - (* stm_match_sum *)
-        rewrite wp_demonic_match_sum.
         apply rule_stm_match_sum; cbn; intros;
           apply rule_pull; intro Heval; rewrite Heval.
         + now apply IHs1.
         + now apply IHs2.
 
       - (* stm_match_prod *)
-        rewrite wp_demonic_match_prod.
         apply rule_stm_match_prod; cbn; intros;
           apply rule_pull; intro Heval; rewrite Heval.
         now apply IHs.
 
       - (* stm_match_enum *)
-        rewrite wp_demonic_match_enum.
         now apply rule_stm_match_enum, H.
 
       - (* stm_match_tuple *)
-        rewrite wp_demonic_match_tuple.
         now apply rule_stm_match_tuple, IHs.
 
       - (* stm_match_union *)
-        rewrite wp_demonic_match_union.
         apply rule_stm_match_union; cbn; intros;
           apply rule_pull; intro Heval; rewrite Heval, unionv_unfold_fold.
         now apply H.
 
       - (* stm_match_record *)
-        rewrite wp_demonic_match_record.
         now apply rule_stm_match_record, IHs.
 
       - (* stm_match_bvec *)
-        rewrite wp_demonic_match_bvec.
         now apply rule_stm_match_bvec, H.
 
       - (* stm_match_bvec_split *)
-        rewrite wp_demonic_match_bvec_split.
         apply rule_stm_match_bvec_split; cbn; intros;
           apply rule_pull; intro Heval.
         now rewrite Heval, bv.appView_app.
@@ -483,20 +208,12 @@ Module Type Soundness
       CHeapSpecM.vcgen n c body ->
       ProgramLogic.ValidContract c body.
     Proof.
-      unfold CHeapSpecM.vcgen, ProgramLogic.ValidContract.
+      rewrite CHeapSpecM.vcgen_equiv.
+      unfold CHeapSpecM.vcgen', ProgramLogic.ValidContract.
       unfold inst_contract_localstore.
-      unfold exec_contract, bind.
       destruct c as [Σ δΣ req result ens]; cbn; intros HYP ι.
-      rewrite env.Forall_forall in HYP.
-      - specialize (HYP ι). remember (inst δΣ ι) as δ.
-        rewrite produce_sound in HYP.
-        apply lwand_sep_adjoint in HYP.
-        rewrite lsep_true in HYP.
-        eapply rule_consequence_left.
-        apply exec_sound. rewrite HYP.
-        apply exec_monotonic. intros v δ1.
-        rewrite consume_sound.
-        now rewrite lsep_comm, lsep_true.
+      eapply rule_consequence_left.
+      apply exec_sound. apply HYP.
     Qed.
 
     Lemma shallow_vcgen_soundness {Δ τ} (c : SepContract Δ τ) (body : Stm Δ τ) :
@@ -504,7 +221,7 @@ Module Type Soundness
       ProgramLogic.ValidContract c body.
     Proof. apply vcgen_sound. Qed.
 
-    (* Print Assumptions shallow_vcgen_soundnes. *)
+    (* Print Assumptions shallow_vcgen_soundness. *)
 
   End Soundness.
 
