theories/Staging/NewShallow/IrisInstance.v
@@ -1,0 +1,1231 @@
+(******************************************************************************)
+(* Copyright (c) 2020 Dominique Devriese, Sander Huyghebaert, Steven Keuchel  *)
+(* All rights reserved.                                                       *)
+(*                                                                            *)
+(* Redistribution and use in source and binary forms, with or without         *)
+(* modification, are permitted provided that the following conditions are     *)
+(* met:                                                                       *)
+(*                                                                            *)
+(* 1. Redistributions of source code must retain the above copyright notice,  *)
+(*    this list of conditions and the following disclaimer.                   *)
+(*                                                                            *)
+(* 2. Redistributions in binary form must reproduce the above copyright       *)
+(*    notice, this list of conditions and the following disclaimer in the     *)
+(*    documentation and/or other materials provided with the distribution.    *)
+(*                                                                            *)
+(* THIS SOFTWARE IS PROVIDED BY THE COPYRIGHT HOLDERS AND CONTRIBUTORS        *)
+(* "AS IS" AND ANY EXPRESS OR IMPLIED WARRANTIES, INCLUDING, BUT NOT LIMITED  *)
+(* TO, THE IMPLIED WARRANTIES OF MERCHANTABILITY AND FITNESS FOR A PARTICULAR *)
+(* PURPOSE ARE DISCLAIMED. IN NO EVENT SHALL THE COPYRIGHT HOLDER OR          *)
+(* CONTRIBUTORS BE LIABLE FOR ANY DIRECT, INDIRECT, INCIDENTAL, SPECIAL,      *)
+(* EXEMPLARY, OR CONSEQUENTIAL DAMAGES (INCLUDING, BUT NOT LIMITED TO,        *)
+(* PROCUREMENT OF SUBSTITUTE GOODS OR SERVICES; LOSS OF USE, DATA, OR         *)
+(* PROFITS; OR BUSINESS INTERRUPTION) HOWEVER CAUSED AND ON ANY THEORY OF     *)
+(* LIABILITY, WHETHER IN CONTRACT, STRICT LIABILITY, OR TORT (INCLUDING       *)
+(* NEGLIGENCE OR OTHERWISE) ARISING IN ANY WAY OUT OF THE USE OF THIS         *)
+(* SOFTWARE, EVEN IF ADVISED OF THE POSSIBILITY OF SUCH DAMAGE.               *)
+(******************************************************************************)
+
+From Equations Require Import
+     Equations Signature.
+Require Import Equations.Prop.EqDec.
+
+From stdpp Require finite gmap list.
+
+From iris Require Import
+     algebra.auth
+     algebra.excl
+     algebra.gmap
+     base_logic.lib.fancy_updates
+     base_logic.lib.gen_heap
+     base_logic.lib.own
+     bi.big_op
+     bi.interface
+     program_logic.adequacy
+     program_logic.weakestpre
+     proofmode.tactics.
+
+From Katamaran Require Import
+     Iris.Model
+     Prelude
+     Semantics
+     Sep.Logic
+     Signature
+     SmallStep.Inversion
+     SmallStep.Step
+     Specification
+     Staging.NewShallow.Executor.
+
+Import ctx.notations.
+Import env.notations.
+
+Set Implicit Arguments.
+
+(* The following three modules define the Iris instance of the program logic
+   depending solely on the operational semantics (through IrisBase) and the
+   user-defined predicates (in IrisPredicates), but without depending on a
+   Specification module. The program logic rules of this subset are implemented
+   in IrisSignatureRules, which is combined with IrisPredicates to form
+   IrisInstance.
+
+   This split allows us to use multiple different specifications with the same
+   Iris model, so that the resulting triples can be combined. This is important
+   particularly when combining specifications of universal contracts for unknown
+   code with known code verifications, e.g. as in the RiscvPmp.BlockVerification
+   proofs. *)
+Module Type IrisPredicates
+  (Import B    : Base)
+  (Import PROG : Program B)
+  (Import SEM  : Semantics B PROG)
+  (Import SIG  : Signature B)
+  (Import IB   : IrisBase B PROG SEM).
+  Parameter luser_inst : forall `{sRG : sailRegGS Σ} `{invGS Σ} (mG : memGS Σ) (p : 𝑯) (ts : Env Val (𝑯_Ty p)), iProp Σ.
+  Parameter lduplicate_inst : forall `{sRG : sailRegGS Σ} `{invGS Σ} (mG : memGS Σ) (p : 𝑯) (ts : Env Val (𝑯_Ty p)),
+      is_duplicable p = true -> bi_entails (luser_inst (sRG := sRG) mG ts) (luser_inst (sRG := sRG) mG ts ∗ luser_inst (sRG := sRG) mG ts).
+
+End IrisPredicates.
+
+Module Type IrisSignatureRules
+  (Import B     : Base)
+  (Import PROG  : Program B)
+  (Import SEM   : Semantics B PROG)
+  (Import SIG   : Signature B)
+  (Import IB    : IrisBase B PROG SEM)
+  (Import IPred : IrisPredicates B PROG SEM SIG IB).
+Section Soundness.
+
+  Import SmallStepNotations.
+
+  Context `{sG : sailGS Σ}.
+
+  #[export] Instance PredicateDefIProp : PredicateDef (IProp Σ) :=
+    {| lptsreg σ r v        := reg_pointsTo r v;
+       luser p ts           := luser_inst sailGS_memGS ts;
+       lduplicate p ts Hdup := lduplicate_inst (sRG := sailGS_sailRegGS) sailGS_memGS ts Hdup
+    |}.
+
+  Lemma reg_valid regstore {τ} (r : 𝑹𝑬𝑮 τ) (v : Val τ) :
+    ⊢ (regs_inv regstore -∗ reg_pointsTo r v -∗ ⌜read_register regstore r = v⌝)%I.
+  Proof.
+    iDestruct 1 as (regsmap) "[Hregs %]".
+    iIntros "Hreg".
+    iDestruct (own_valid_2 with "Hregs Hreg") as %[Hl regsv]%auth_both_valid.
+    iPureIntro.
+    specialize (Hl 0).
+    setoid_rewrite (singleton_includedN_l 0 regsmap (existT _ r) _) in Hl.
+    destruct Hl as [y [eq1%discrete%leibniz_equiv eq2%cmra_discrete_included_r]];
+      auto with typeclass_instances.
+    specialize (regsv (existT _ r)).
+    rewrite eq1 in regsv.
+    destruct y as [y|]; [|inversion regsv].
+    setoid_rewrite Excl_included in eq2.
+    apply leibniz_equiv in eq2. subst.
+    specialize (H (existT _ r) (Excl (existT _ v)) eq1); cbn in H.
+    Local Set Equations With UIP.
+    by dependent elimination H.
+  Qed.
+
+  Lemma regs_inv_update {τ} {r} {v : Val τ} {regsmap : gmapUR SomeReg (exclR (leibnizO SomeVal))} {regstore : RegStore} :
+    map_Forall (K := SomeReg) (A := excl SomeVal) (λ r' v', match r' with
+                         | existT τ r'' => Excl (existT _ (read_register regstore r'')) = v'
+                         end) regsmap ->
+    (own reg_gv_name (● <[existT _ r:=Excl (existT _ v)]> regsmap)) -∗ regs_inv (write_register regstore r v).
+  Proof.
+    iIntros (regseq) "Hownregs".
+    iExists (<[existT _ r:=Excl (existT _ v)]> regsmap).
+    iFrame.
+    iPureIntro.
+    apply (map_Forall_lookup_2 _ (<[existT _ r:=Excl (existT _ v)]> regsmap)).
+    intros [τ' r'] x eq1.
+    destruct (eq_dec_het r r') as [eq2|neq].
+    + dependent elimination eq2.
+      rewrite lookup_insert in eq1.
+      apply (inj Some) in eq1.
+      by rewrite <- eq1, (read_write regstore r v).
+    + assert (existT _ r ≠ existT _ r') as neq2.
+      * intros eq2.
+        dependent elimination eq2.
+        now apply neq.
+      * rewrite (lookup_insert_ne _ _ _ _ neq2) in eq1.
+        rewrite (read_write_distinct _ _ neq).
+        apply (map_Forall_lookup_1 _ _ _ _ regseq eq1).
+  Qed.
+
+  Lemma reg_update regstore {τ} r (v1 v2 : Val τ) :
+    regs_inv regstore -∗ reg_pointsTo r v1 ==∗ regs_inv (write_register regstore r v2) ∗ reg_pointsTo r v2.
+  Proof.
+    iDestruct 1 as (regsmap) "[Hregs %]".
+    rewrite /reg_pointsTo.
+    iIntros "Hreg".
+    iDestruct (own_valid_2 with "Hregs Hreg") as %[Hl%cmra_discrete_included_r regsmapv]%auth_both_valid.
+    setoid_rewrite (singleton_included_l regsmap (existT _ r) _) in Hl.
+    destruct Hl as [y [eq1%leibniz_equiv eq2]].
+    specialize (regsmapv (existT _ r)).
+    rewrite eq1 in regsmapv.
+    destruct y as [y|]; inversion regsmapv.
+    iMod (own_update_2 with "Hregs Hreg") as "[Hregs Hreg]".
+    {
+      eapply auth_update.
+      apply (singleton_local_update regsmap (existT _ r) (Excl y) (Excl (existT _ v1)) (Excl (existT _ v2)) (Excl (existT _ v2)) eq1).
+      by eapply exclusive_local_update.
+    }
+    iModIntro.
+    iFrame.
+    iApply (regs_inv_update H); iFrame.
+  Qed.
+
+  Definition semWP [Γ τ] (s : Stm Γ τ)
+    (POST : Val τ → CStore Γ → iProp Σ) (δ : CStore Γ) : iProp Σ :=
+    WP {| conf_stm := s; conf_store := δ |} ?{{ v, POST (valconf_val v) (valconf_store v) }}.
+
+  Lemma semWP_mono [Γ τ] (s : Stm Γ τ) (P Q : Val τ → CStore Γ → iProp Σ) :
+    (forall v δ, P v δ -∗ Q v δ) -> (forall δ, semWP s P δ -∗ semWP s Q δ).
+  Proof.
+    unfold semWP. intros PQ δ.
+    apply wp_mono. now intros [].
+  Qed.
+
+  Lemma semWP_strong_mono [Γ τ] (s : Stm Γ τ) (P Q : Val τ → CStore Γ → iProp Σ) (δ : CStore Γ) :
+    ⊢ (∀ v δ, P v δ -∗ Q v δ) -∗ (semWP s P δ -∗ semWP s Q δ).
+  Proof.
+    unfold semWP. iIntros "PQ WP".
+    iApply (wp_strong_mono with "WP"); auto.
+    iIntros ([v δΓ]) "X"; cbn.
+    iModIntro. by iApply "PQ".
+  Qed.
+
+  Definition ValidLemma {Δ} (lem : Lemma Δ) : Prop :=
+    match lem with
+      {| lemma_logic_variables := Σ;
+         lemma_patterns        := θΔ;
+         lemma_precondition    := req;
+         lemma_postcondition   := ens;
+      |} =>
+      forall (ι : Valuation Σ),
+        ⊢ asn.interpret req ι -∗
+          asn.interpret ens ι
+    end.
+
+  Fixpoint Forall {Δ : LCtx} {struct Δ} : (Valuation Δ -> iProp Σ) -> iProp Σ :=
+    match Δ return (Valuation Δ -> iProp Σ) -> iProp Σ with
+    | ctx.nil      => fun P => P env.nil
+    | ctx.snoc Δ b => fun P => Forall (fun δ => ∀ (v : Val (type b)), P (env.snoc δ b v))
+    end%I.
+
+  (* Lemma iris_rule_consequence {Γ σ} {δ : CStore Γ} *)
+  (*       {P P'} {Q Q' : Val σ -> CStore Γ -> iProp Σ} {s : Stm Γ σ} : *)
+  (*       (P ⊢ P') -> (forall v δ', Q' v δ' ⊢ Q v δ') -> *)
+  (*       semTriple δ P' s Q' -∗ semTriple δ P s Q. *)
+  (* Proof. *)
+  (*   iIntros (PP QQ) "trips P". *)
+  (*   iApply (wp_mono _ _ _ (fun v => match v with MkValConf _ v δ' => Q' v δ' end)). *)
+  (*   + intros [v δ']; cbn. *)
+  (*     apply QQ. *)
+  (*   + iApply "trips". *)
+  (*     iApply PP; iFrame. *)
+  (* Qed. *)
+
+  (* Lemma iris_rule_frame {Γ σ} {δ : CStore Γ} *)
+  (*       (R P : iProp Σ) (Q : Val σ -> CStore Γ -> iProp Σ) (s : Stm Γ σ) : *)
+  (*       (⊢ semTriple δ P s Q -∗ semTriple δ (R ∗ P) s (fun v δ' => R ∗ Q v δ'))%I. *)
+  (* Proof. *)
+  (*   iIntros "trips [HR HP]". *)
+  (*   iApply (wp_frame_l _ _ (MkConf s δ) (fun v => match v with MkValConf _ v δ' => Q v δ' end) R). *)
+  (*   iFrame. *)
+  (*   by iApply "trips". *)
+  (* Qed. *)
+
+  (* Lemma iris_rule_pull {σ Γ} (δ : CStore Γ) (s : Stm Γ σ) *)
+  (*       (P : iProp Σ) (Q : Prop) (R : Val σ -> CStore Γ -> iProp Σ) : *)
+  (*       (⊢ (⌜ Q ⌝ → semTriple δ P s R) -∗ semTriple δ (P ∧ bi_pure Q) s R)%I. *)
+  (* Proof. *)
+  (*   iIntros "QP [P %]". *)
+  (*   by iApply "QP". *)
+  (* Qed. *)
+
+  (* Lemma iris_rule_exist {σ Γ} (δ : CStore Γ) *)
+  (*       (s : Stm Γ σ) {A : Type} {P : A -> iProp Σ} *)
+  (*       {Q :  Val σ -> CStore Γ -> iProp Σ} : *)
+  (*       ⊢ ((∀ x, semTriple δ (P x) s Q) -∗ semTriple δ (∃ x, P x) s Q)%I. *)
+  (* Proof. *)
+  (*   iIntros "trips Px". *)
+  (*   iDestruct "Px" as (x) "Px". *)
+  (*   by iApply "trips". *)
+  (* Qed. *)
+
+  Definition semTriple {Γ τ} (δ : CStore Γ) (PRE : iProp Σ) (s : Stm Γ τ)
+    (POST : Val τ -> CStore Γ -> iProp Σ) : iProp Σ :=
+    PRE -∗ semWP s POST δ.
+  (* always modality needed? perhaps not because sail not higher-order? *)
+
+  (* Lemma iris_rule_noop {Γ σ} {δ : CStore Γ} *)
+  (*       {P} {Q : Val σ -> CStore Γ -> iProp Σ} {s : Stm Γ σ} : *)
+  (*   language.to_val (MkConf s δ) = None -> *)
+  (*   (forall {s' γ γ' μ μ' δ'}, ⟨ γ, μ, δ, s ⟩ ---> ⟨ γ', μ', δ', s' ⟩ -> *)
+  (*                           (γ' = γ) /\ (μ' = μ) /\ (δ' = δ) /\ *)
+  (*                           ((exists v, s' = stm_val _ v) \/ (exists msg, s' = stm_fail _ msg))) -> *)
+  (*   (∀ v, P ={⊤}=∗ Q v δ) -∗ *)
+  (*                semTriple δ P s Q. *)
+  (* Proof. *)
+  (*   iIntros (Hnv Hnoop) "HPQ HP". *)
+  (*   rewrite wp_unfold. *)
+  (*   unfold wp_pre. *)
+  (*   rewrite Hnv. cbn. *)
+  (*   iIntros (σ' ns ks1 ks nt) "Hregs". *)
+  (*   iMod (fupd_mask_subseteq empty) as "Hclose"; first set_solver. *)
+  (*   iModIntro. *)
+  (*   iSplitR; first done. *)
+  (*   iIntros (e2 σ'' efs) "%". *)
+  (*   dependent elimination H. *)
+  (*   destruct (Hnoop _ _ _ _ _ _ s0) as (-> & -> & -> & [[v ->]|[msg ->]]). *)
+  (*   - do 3 iModIntro. *)
+  (*     iMod "Hclose" as "_". *)
+  (*     iMod ("HPQ" with "HP") as "HQ". *)
+  (*     iModIntro. *)
+  (*     iFrame. *)
+  (*     iSplitL; trivial. *)
+  (*     now iApply wp_value. *)
+  (*   - do 3 iModIntro. *)
+  (*     iMod "Hclose" as "_". *)
+  (*     iModIntro. *)
+  (*     iFrame. *)
+  (*     iSplitL; trivial. *)
+  (*     now iApply wp_compat_fail. *)
+  (* Qed. *)
+
+End Soundness.
+
+Section Adequacy.
+
+  Import SmallStepNotations.
+
+  Definition sailΣ : gFunctors := #[ memΣ ; invΣ ; GFunctor regUR].
+
+  Instance subG_sailGpreS {Σ} : subG sailΣ Σ -> sailGpreS Σ.
+  Proof.
+    intros.
+    lazymatch goal with
+    | H:subG ?xΣ _ |- _ => try unfold xΣ in H
+    end.
+    repeat match goal with
+           | H:subG (gFunctors.app _ _) _ |- _ => apply subG_inv in H; destruct H
+           end.
+    split; eauto using memΣ_GpreS, subG_invΣ.
+    solve_inG.
+ Qed.
+
+  Definition RegStore_to_map (γ : RegStore) : gmap SomeReg (exclR (leibnizO SomeVal)) :=
+    list_to_map (K := SomeReg)
+                (fmap (fun x => match x with
+                              existT _ r =>
+                                pair (existT _ r) (Excl (existT _ (read_register γ r)))
+                            end)
+                     (finite.enum (sigT 𝑹𝑬𝑮))).
+
+  Lemma RegStore_to_map_Forall (γ : RegStore) :
+    map_Forall (K := SomeReg)
+      (fun reg v => match reg with | existT _ reg => Excl (existT _ (read_register γ reg)) = v end)
+      (RegStore_to_map γ).
+  Proof.
+    eapply map_Forall_lookup_2.
+    intros [σ r] x eq.
+    unfold RegStore_to_map in eq.
+    remember (list_to_map _ !! _) as o in eq.
+    destruct o; inversion eq; subst.
+    assert (eq' := eq_sym Heqo).
+    rewrite <-elem_of_list_to_map in eq'.
+    - eapply elem_of_list_fmap_2 in eq'.
+      destruct eq' as ([σ' r'] & eq2 & eq3).
+      now inversion eq2.
+    - rewrite <-list_fmap_compose.
+      rewrite (list_fmap_ext (compose fst (λ x : {H : Ty & 𝑹𝑬𝑮 H},
+          let (x0, r0) := x in (existT x0 r0 , Excl (existT x0 (read_register γ r0))))) id _ _ _ eq_refl).
+      + rewrite list_fmap_id.
+        eapply finite.NoDup_enum.
+      + now intros [σ' r'].
+  Qed.
+
+  Lemma RegStore_to_map_valid (γ : RegStore) :
+    valid (RegStore_to_map γ).
+  Proof.
+    intros i.
+    cut (exists v, RegStore_to_map γ !! i = Some (Excl v)).
+    - intros [v eq].
+      now rewrite eq.
+    - destruct i as [σ r].
+      exists (existT _ (read_register γ r)).
+      eapply elem_of_list_to_map_1'.
+      + intros y eq.
+        eapply elem_of_list_fmap_2 in eq.
+        destruct eq as ([σ2 r2] & eq1 & eq2).
+        now inversion eq1.
+      + refine (elem_of_list_fmap_1 _ _ (existT _ r) _).
+        eapply finite.elem_of_enum.
+  Qed.
+
+  Lemma steps_to_erased {σ Γ γ μ δ} (s : Stm Γ σ) {γ' μ' δ' s'}:
+    ⟨ γ, μ, δ, s ⟩ --->* ⟨ γ', μ', δ', s' ⟩ ->
+    rtc erased_step (cons (MkConf s δ) nil, (γ,μ)) (cons (MkConf s' δ') nil, (γ',μ')).
+  Proof.
+    induction 1; first done.
+    refine (rtc_l _ _ _ _ _ IHSteps).
+    exists nil.
+    refine (step_atomic _ _ _ _ _ nil nil eq_refl eq_refl _).
+    by eapply mk_prim_step.
+  Qed.
+
+  Lemma own_RegStore_to_map_reg_pointsTos `{sailRegGS Σ'} {γ : RegStore} {l : list (sigT 𝑹𝑬𝑮)} :
+    NoDup l ->
+    ⊢ own reg_gv_name (◯ list_to_map (K := SomeReg)
+                         (fmap (fun x => match x with existT _ r =>
+                                                     pair (existT _ r) (Excl (existT _ (read_register γ r)))
+                                      end) l)) -∗
+      [∗ list] x ∈ l,
+        let (x0, r) := (x : sigT 𝑹𝑬𝑮) in reg_pointsTo r (read_register γ r).
+  Proof.
+    iIntros (nodups) "Hregs".
+    iInduction l as [|[x r]] "IH".
+    - now iFrame.
+    - rewrite big_sepL_cons. cbn.
+      rewrite (insert_singleton_op (A := exclR (leibnizO SomeVal)) (list_to_map (_ <$> l))  (existT x r) (Excl (existT _ (read_register γ r)))).
+      rewrite auth_frag_op.
+      iPoseProof (own_op with "Hregs") as "[Hreg Hregs]".
+      iFrame.
+      iApply "IH".
+      + iPureIntro.
+        refine (NoDup_cons_1_2 (existT x r) l nodups).
+      + iFrame.
+      + destruct (proj1 (NoDup_cons (existT x r) _) nodups) as [notin _].
+        refine (not_elem_of_list_to_map_1 _ (existT x r) _).
+        rewrite <-list_fmap_compose.
+        rewrite (list_fmap_ext (compose fst (λ x : {H : Ty & 𝑹𝑬𝑮 H},
+          let (x0, r0) := x in (existT x0 r0, Excl (existT x0 (read_register γ r0))))) id _ _ _ eq_refl).
+        now rewrite list_fmap_id.
+        now intros [σ2 r2].
+  Qed.
+
+  Lemma adequacy {Γ σ} (s : Stm Γ σ) {γ γ'} {μ μ'}
+        {δ δ' : CStore Γ} {s' : Stm Γ σ} {Q : Val σ -> Prop} :
+    ⟨ γ, μ, δ, s ⟩ --->* ⟨ γ', μ', δ', s' ⟩ -> Final s' ->
+    (forall `{sailGS Σ'},
+        ⊢ semTriple (Σ := Σ') δ
+          (mem_res sailGS_memGS μ ∗
+           [∗ list] _ ↦ x ∈ finite.enum (sigT 𝑹𝑬𝑮),
+              match x with | existT _ r => reg_pointsTo r (read_register γ r) end
+          )%I s (fun v δ' => bi_pure (Q v)))%I ->
+    ResultOrFail s' Q.
+  Proof.
+    intros steps fins trips.
+    cut (adequate MaybeStuck (MkConf s δ) (γ,μ)
+             (λ (v : val (microsail_lang Γ σ)) (_ : state (microsail_lang Γ σ)),
+                (λ v0 : val (microsail_lang Γ σ), match v0 with
+                                                  | MkValConf _ v' _ => Q v'
+                                                  end) v)).
+    - destruct s'; cbn in fins; destruct fins; last done.
+      intros adeq.
+      apply (adequate_result MaybeStuck (MkConf s δ) (γ , μ) (fun v _ => match v with | MkValConf _ v' δ' => Q v' end) adeq nil (γ' , μ') (MkValConf _ v δ')).
+      by apply steps_to_erased.
+    - constructor; last done.
+      intros t2 σ2 [v2 δ2] eval.
+      assert (eq := RegStore_to_map_Forall γ).
+      assert (regsmapv := RegStore_to_map_valid γ).
+      pose proof (wp_adequacy sailΣ (microsail_lang Γ σ) MaybeStuck (MkConf s δ) (γ , μ) (fun v => match v with | MkValConf _ v' δ' => Q v' end)) as adeq.
+      refine (adequate_result _ _ _ _ (adeq _) _ _ _ eval); clear adeq.
+      iIntros (Hinv κs) "".
+      iMod (own_alloc ((● RegStore_to_map γ ⋅ ◯ RegStore_to_map γ ) : regUR)) as (spec_name) "[Hs1 Hs2]";
+        first by apply auth_both_valid.
+      pose proof (memΣ_GpreS (Σ := sailΣ) _) as mPG.
+      iMod (mem_inv_init μ mPG) as (memG) "[Hmem Rmem]".
+      iModIntro.
+      iExists (fun σ _ => regs_inv (H := (SailRegGS _ spec_name)) (σ.1) ∗ mem_inv memG (σ.2))%I.
+      iExists _.
+      iSplitR "Hs2 Rmem".
+      * iSplitL "Hs1".
+        + iExists (RegStore_to_map γ).
+          by iFrame.
+        + iFrame.
+      * iPoseProof (trips sailΣ (SailGS Hinv (SailRegGS reg_pre_inG spec_name) memG) with "[Rmem Hs2]") as "trips'".
+        + iFrame.
+          unfold RegStore_to_map.
+          iApply (own_RegStore_to_map_reg_pointsTos (H := SailRegGS reg_pre_inG spec_name)(γ := γ) (l := finite.enum (sigT 𝑹𝑬𝑮)) with "Hs2").
+          eapply finite.NoDup_enum.
+        + iApply (wp_mono with "trips'").
+          by iIntros ([δ3 v]).
+  Qed.
+End Adequacy.
+End IrisSignatureRules.
+
+Module Type IrisInstance (B : Base) (PROG : Program B) (SEM : Semantics B PROG) (SIG : Signature B) (IB : IrisBase B PROG SEM) :=
+  IrisPredicates B PROG SEM SIG IB <+ IrisSignatureRules B PROG SEM SIG IB.
+
+(*
+ * The following module defines the parts of the Iris model that must depend on the Specification, not just on the Signature.
+ * This is kept to a minimum (see comment for the IrisPredicates module).
+ *)
+Module IrisInstanceWithContracts
+  (Import B     : Base)
+  (Import PROG  : Program B)
+  (Import SEM   : Semantics B PROG)
+  (Import SIG   : Signature B)
+  (Import SPEC  : Specification B PROG SIG)
+  (Import IB    : IrisBase B PROG SEM)
+  (Import II    : IrisInstance B PROG SEM SIG IB)
+  (Import NS    : NewShallowExecOn B PROG SIG SPEC).
+
+  Section WithSailGS.
+  Context {Σ} {sG : sailGS Σ}.
+
+  Definition ForeignSem : Prop :=
+    ∀ (Γ : PCtx) (Δ : PCtx) (τ : Ty) (f : 𝑭𝑿 Δ τ) (es : NamedEnv (Exp Γ) Δ)
+      (POST : Val τ → CStore Γ → iProp Σ) (δΓ : CStore Γ),
+      CPureSpecM.call_contract (CEnvEx f) (evals es δΓ) (fun v => POST v δΓ) -∗
+      semWP (stm_foreign f es) POST δΓ.
+
+  Definition LemmaSem : Prop :=
+    forall (Δ : PCtx) (l : 𝑳 Δ),
+      ValidLemma (LEnv l).
+
+  Ltac fold_semWP :=
+    first
+      [ progress
+          change_no_check
+          (wp MaybeStuck top
+              {| conf_stm := ?s; conf_store := ?δ |}
+              (fun v => ?POST (valconf_val v) (valconf_store v)))
+        with (semWP s POST δ)
+      | progress
+          change_no_check
+          (wp MaybeStuck top
+              {| conf_stm := ?s; conf_store := ?δ |}
+              ?POST)
+        with (semWP s (fun v δ' => POST (MkValConf _ v δ')) δ);
+        try (progress (cbn [valconf_val valconf_store]))
+      ].
+
+  Definition semCall [Δ τ] (f : 𝑭 Δ τ) (args : CStore Δ) (Q : Val τ -> iProp Σ) :
+    iProp Σ := ▷ CHeapSpecM.exec_call_inline semWP f args Q.
+
+  Definition semWP' [Γ τ] (s : Stm Γ τ) :
+    (Val τ -> CStore Γ -> iProp Σ) -> CStore Γ -> iProp Σ :=
+    CHeapSpecM.exec_open semWP semCall s.
+  Arguments semWP' : simpl never.
+
+  Definition ref {Γ1 Γ2 A}
+    (F G : (A → CStore Γ2 → iProp Σ) → CStore Γ1 → iProp Σ) : iProp Σ :=
+    ∀ (POST : A → CStore Γ2 → iProp Σ) (δ : CStore Γ1),
+      F POST δ -∗ G POST δ.
+  Notation "F ≼ G" := (ref F G).
+
+  Lemma semWP_val {Γ τ} (v : Val τ) (POST : Val τ → CStore Γ → iProp Σ) (δ : CStore Γ) :
+    semWP (stm_val τ v) POST δ ⊣⊢ |={⊤}=> POST v δ.
+  Proof. unfold semWP. rewrite wp_unfold. reflexivity. Qed.
+
+  Lemma rule_val {Γ τ} (v : Val τ) :
+    ⊢ semWP' (Γ := Γ) (stm_val τ v) ≼ semWP (stm_val τ v).
+  Proof. iIntros (POST δ). rewrite semWP_val; auto. Qed.
+
+  Lemma rule_exp {Γ τ} (e : Exp Γ τ) :
+    ⊢ semWP' (stm_exp e) ≼ semWP (stm_exp e).
+  Proof.
+    iIntros (POST δ) "P". unfold semWP.
+    iApply (wp_mask_mono _ empty); auto.
+    rewrite wp_unfold.
+    iIntros ([regs μ] ns k ks nt) "[Hregs Hmem]".
+    iModIntro.
+    iSplitR; [trivial|].
+    iIntros (e2 σ2 efs) "%".
+    remember (MkConf (stm_exp e) δ) as t.
+    destruct H.
+    dependent elimination Heqt.
+    dependent elimination H. cbn.
+    iModIntro. iModIntro. iModIntro.
+    iFrame.
+    iSplitL; trivial.
+    by iApply wp_value.
+  Qed.
+
+  Lemma semWP_fail {Γ τ s} (POST : Val τ → CStore Γ → iProp Σ) (δ : CStore Γ) :
+    semWP (stm_fail _ s) POST δ ⊣⊢ True.
+  Proof.
+    apply bi.entails_anti_sym.
+    - auto.
+    - iIntros "_".
+      unfold semWP. rewrite wp_unfold. cbn.
+      iIntros (σ _ ks1 ks nt) "Hregs".
+      iMod (fupd_mask_subseteq empty) as "Hclose"; first set_solver.
+      iModIntro.
+      iSplitR; [trivial|].
+      iIntros (e2 σ2 efs) "%".
+      remember (MkConf (fail s) δ) as s1.
+      destruct H.
+      inversion Heqs1. subst.
+      inversion H.
+  Qed.
+
+  Lemma rule_fail {Γ τ s} :
+    ⊢ semWP' (Γ := Γ) (stm_fail τ s) ≼ semWP (stm_fail τ s).
+  Proof. iIntros (POST δ) "_". rewrite semWP_fail; auto. Qed.
+
+  Lemma rule_bind {Γ τ σ} (s : Stm Γ σ) (k : Val σ → Stm Γ τ) :
+    ⊢ semWP' (stm_bind s k) ≼ semWP (stm_bind s k).
+  Proof.
+    iIntros (POST). iRevert (s). iLöb as "IH". iIntros (s δ) "WPs".
+    unfold semWP at 2. rewrite wp_unfold. cbn.
+    iIntros ([regs μ] ns ks1 ks nt) "Hregs".
+    iMod (fupd_mask_subseteq empty) as "Hclose"; first set_solver.
+    iModIntro.
+    iSplitR; [trivial|].
+    iIntros (e2 [regs2 μ2] efs) "%".
+    dependent elimination H.
+    fold_semWP.
+    dependent elimination s0.
+    + unfold semWP'; cbn.
+      unfold semWP at 4. rewrite wp_unfold.
+      unfold wp_pre.
+      rewrite (val_stuck (MkConf s13 δ1) (γ1 , μ1) [] _ _ [] (mk_prim_step s14)).
+      iSpecialize ("WPs" $! (γ1 , μ1) ns nil nil nt with "Hregs"). cbn.
+      iMod "Hclose".
+      iMod "WPs" as "[_ WPs]".
+      iSpecialize ("WPs" $! _ _ nil (mk_prim_step s14)).
+      iMod "WPs" as "WPs".
+      iModIntro. iModIntro.
+      iMod "WPs".
+      iModIntro.
+      iMod "WPs" as "[Hregs [wps _]]".
+      fold_semWP.
+      iModIntro.
+      iFrame.
+      by iApply "IH".
+    + iModIntro. iModIntro. iModIntro.
+      iMod "Hclose" as "_".
+      unfold semWP', CHeapSpecM.exec_open; cbn.
+      rewrite semWP_val.
+      iMod "WPs" as "WPs".
+      iModIntro.
+      by iFrame.
+    + iModIntro. iModIntro. iModIntro.
+      iMod "Hclose" as "_".
+      iFrame; iSplitL; auto.
+      by iApply semWP_fail.
+  Qed.
+
+  Lemma rule_block {Γ τ Δ} (δΔ : CStore Δ) (s : Stm (Γ ▻▻ Δ) τ) :
+    ⊢ semWP' (stm_block δΔ s) ≼ semWP (stm_block δΔ s).
+  Proof.
+    iIntros (POST). iRevert (δΔ s).
+    iLöb as "IH". iIntros (δΔ k δΓ) "WPk".
+    unfold semWP at 2. rewrite wp_unfold. cbn.
+    iIntros (σ ns ks1 ks nt) "state_inv".
+    iMod (fupd_mask_subseteq empty) as "Hclose"; first set_solver.
+    iModIntro.
+    iSplitR; [trivial|].
+    iIntros (e2 [regs2 μ2] efs) "%".
+    dependent elimination H.
+    fold_semWP.
+    dependent elimination s.
+    - iModIntro. iModIntro. iModIntro.
+      iMod "Hclose" as "_".
+      unfold semWP', CHeapSpecM.exec_open, CHeapSpecM.pushspops.
+      rewrite semWP_val.
+      rewrite env.drop_cat.
+      iMod "WPk" as "WPk".
+      iModIntro.
+      iFrame.
+      iSplitL; [|trivial].
+      by iApply semWP_val.
+    - iModIntro. iModIntro. iModIntro.
+      iMod "Hclose" as "_".
+      iFrame; iSplitL; auto.
+      by iApply semWP_fail.
+    - unfold semWP', CHeapSpecM.exec_open, CHeapSpecM.pushspops.
+      unfold semWP at 3. rewrite wp_unfold. cbn.
+      unfold wp_pre.
+      rewrite (val_stuck (MkConf k1 _) (γ1 , μ1) [] _ _ [] (mk_prim_step s1)).
+      iSpecialize ("WPk" $! (γ1 , μ1) ns nil nil nt with "state_inv"). cbn.
+      iMod "Hclose".
+      iMod "WPk" as "[_ WPk]".
+      iSpecialize ("WPk" $! _ _ nil (mk_prim_step s1)).
+      iMod "WPk" as "WPk".
+      iModIntro. iModIntro.
+      iMod "WPk".
+      iModIntro.
+      iMod "WPk" as "[Hregs [wps _]]".
+      fold_semWP.
+      iModIntro.
+      iFrame.
+      by iApply "IH".
+  Qed.
+
+  Lemma rule_let {Γ τ x σ} (s1 : Stm Γ σ) (s2 : Stm (Γ ▻ x∷σ) τ) :
+    ⊢ semWP' (stm_let x σ s1 s2) ≼ semWP (stm_let x σ s1 s2).
+  Proof.
+    iIntros (POST δ) "WPs". unfold semWP.
+    rewrite wp_unfold. cbn.
+    iIntros ([regs μ] ns ks1 ks nt) "state_inv".
+    iMod (fupd_mask_subseteq empty) as "Hclose"; first set_solver.
+    iModIntro.
+    iSplitR; [trivial|].
+    iIntros (e2 [regs2 μ2] efs) "%".
+    dependent elimination H.
+    fold_semWP.
+    dependent elimination s.
+    iModIntro. iModIntro. iModIntro.
+    iMod "Hclose" as "_".
+    iModIntro.
+    iFrame; iSplitL; auto.
+    iApply rule_bind.
+    unfold semWP', CHeapSpecM.exec_open, CHeapSpecM.bind, CHeapSpecM.pushpop.
+    iApply (semWP_mono with "WPs"); cbn.
+    iIntros (v δ) "wpk".
+    by iApply (rule_block [env].[_∷_ ↦ v]).
+  Qed.
+
+  Lemma rule_assign {Γ τ x} (xInΓ : x∷τ ∈ Γ) (s : Stm Γ τ) :
+    ⊢ semWP' (stm_assign x s) ≼ semWP (stm_assign x s).
+  Proof.
+    iIntros (POST). iRevert (s). iLöb as "IH". iIntros (s δ) "WPs".
+    unfold semWP at 2. rewrite wp_unfold. cbn.
+    iIntros ([regs μ] ns ks1 ks nt) "Hregs".
+    iMod (fupd_mask_subseteq empty) as "Hclose"; first set_solver.
+    iModIntro.
+    iSplitR; [trivial|].
+    iIntros (e2 [regs2 μ2] efs) "%".
+    dependent elimination H.
+    dependent elimination s0; fold_semWP.
+    + iModIntro. iModIntro. iModIntro.
+      unfold semWP' at 2, CHeapSpecM.exec_open, CHeapSpecM.bind, CHeapSpecM.assign, CHeapSpecM.pure.
+      rewrite semWP_val.
+      iMod "Hclose" as "_".
+      iMod "WPs" as "WPs".
+      iModIntro.
+      iFrame.
+      iSplitL; [|trivial].
+      by iApply semWP_val.
+    + iModIntro. iModIntro. iModIntro.
+      iMod "Hclose" as "_".
+      iFrame; iSplitL; auto.
+      by iApply semWP_fail.
+    + unfold semWP' at 2, CHeapSpecM.exec_open, CHeapSpecM.bind, CHeapSpecM.assign, CHeapSpecM.pure.
+      unfold semWP at 2. rewrite wp_unfold. unfold wp_pre.
+      rewrite (val_stuck (MkConf s9 δ1) _ [] _ _ [] (mk_prim_step s10)).
+      iSpecialize ("WPs" $! _ ns nil nil nt with "Hregs"). cbn.
+      iMod "Hclose".
+      iMod "WPs" as "[_ WPs]".
+      iSpecialize ("WPs" $! _ _ nil (mk_prim_step s10)).
+      fold_semWP.
+      iMod "WPs" as "WPs".
+      iModIntro. iModIntro.
+      iMod "WPs".
+      iModIntro.
+      iMod "WPs" as "[Hregs [WPs _]]".
+      iModIntro.
+      iFrame.
+      by iApply "IH".
+  Qed.
+
+  Lemma rule_call_frame {Γ τ Δ} (δΔ : CStore Δ) (s : Stm Δ τ) :
+    ⊢ semWP' (Γ := Γ) (stm_call_frame δΔ s) ≼ semWP (stm_call_frame δΔ s).
+  Proof.
+    iIntros (POST δΓ). iRevert (δΔ s).
+    iLöb as "IH". iIntros (δΔ s) "WPs".
+    unfold semWP at 2. rewrite wp_unfold. cbn.
+    iIntros (σ ns ks1 ks nt) "Hregs".
+    iMod (fupd_mask_subseteq empty) as "Hclose"; first set_solver.
+    iModIntro.
+    iSplitR; first trivial.
+    iIntros (e2 σ2 efs) "%".
+    dependent elimination H.
+    fold_semWP.
+    dependent elimination s0.
+    - iMod "Hclose" as "_".
+      unfold semWP' at 2; cbn.
+      unfold semWP at 2.
+      rewrite wp_unfold.
+      rewrite {1}/wp_pre.
+      rewrite (val_stuck (MkConf s5 _) (γ1 , μ1) [] _ _ [] (mk_prim_step s6)).
+      iMod ("WPs" $! (γ1 , μ1) ns nil ks nt with "Hregs") as "[% WPs]". cbn.
+      iMod ("WPs" $! _ _ _ (mk_prim_step s6)) as "WPs".
+      fold_semWP.
+      iModIntro. iModIntro.
+      iMod "WPs".
+      iModIntro.
+      iMod "WPs" as "[Hregs [WPs' _]]".
+      iModIntro.
+      iFrame.
+      iSplitL; last trivial.
+      by iApply "IH".
+    - iModIntro. iModIntro. iModIntro.
+      iMod "Hclose" as "_".
+      iModIntro.
+      iFrame.
+      iSplitL; last trivial.
+      unfold semWP' at 2, CHeapSpecM.exec_open, CHeapSpecM.bind,
+        CHeapSpecM.get_local, CHeapSpecM.put_local.
+      by rewrite ?semWP_val.
+    - iModIntro. iModIntro. iModIntro.
+      iMod "Hclose" as "_".
+      iFrame.
+      iModIntro.
+      iSplitL; [|trivial].
+      by iApply semWP_fail.
+  Qed.
+
+  Lemma semWP_call {Γ τ Δ} (f : 𝑭 Δ τ) (es : NamedEnv (Exp Γ) Δ)
+    (POST : Val τ → CStore Γ → iProp Σ) (δΓ : CStore Γ) :
+    ▷ semWP (FunDef f) (fun vτ _ => POST vτ δΓ) (evals es δΓ) -∗
+    semWP (stm_call f es) POST δΓ.
+  Proof.
+    iIntros "wpbody".
+    unfold semWP at 2.
+    rewrite wp_unfold. cbn.
+    iIntros (σ' ns ks1 ks nt) "Hregs".
+    iMod (fupd_mask_subseteq empty) as "Hclose"; first set_solver.
+    iModIntro. iSplitR; [trivial|].
+    iIntros (e2 σ'' efs) "%".
+    dependent elimination H.
+    fold_semWP.
+    dependent elimination s.
+    iModIntro. iModIntro. iModIntro.
+    iMod "Hclose" as "_".
+    iModIntro. iFrame.
+    iSplitL; [|trivial].
+    by iApply rule_call_frame.
+  Qed.
+
+  Lemma rule_call {Γ τ Δ} (f : 𝑭 Δ τ) (es : NamedEnv (Exp Γ) Δ) :
+    ⊢ semWP' (stm_call f es) ≼ semWP (stm_call f es).
+  Proof.
+    iIntros (POST δ) "WPbody".
+    unfold semWP. rewrite wp_unfold. cbn.
+    iIntros (σ' ns ks1 ks nt) "Hregs".
+    iMod (fupd_mask_subseteq empty) as "Hclose"; first set_solver.
+    iModIntro. iSplitR; [trivial|].
+    iIntros (e2 σ'' efs) "%".
+    dependent elimination H.
+    fold_semWP.
+    dependent elimination s.
+    unfold semWP', semCall. cbn.
+    iModIntro. iModIntro. iModIntro.
+    iMod "Hclose" as "_".
+    iModIntro. iFrame.
+    iSplitL; [|trivial].
+    by iApply rule_call_frame.
+  Qed.
+
+  Lemma rule_foreign {Γ τ Δ} (f : 𝑭𝑿 Δ τ) (es : NamedEnv (Exp Γ) Δ) :
+    ForeignSem ->
+    ⊢ semWP' (stm_foreign f es) ≼ semWP (stm_foreign f es).
+  Proof. iIntros (extSem POST δΓ) "WPs". by iApply extSem. Qed.
+
+  Lemma equiv_call_lemma {Δ} (lem : Lemma Δ) (args : CStore Δ) POST :
+    CPureSpecM.call_lemma lem args POST ⊣⊢ CPureSpecM.call_lemma' lem args POST.
+  Proof. apply bi.entails_anti_sym; apply CPureSpecM.equiv_call_lemma. Qed.
+
+  Lemma rule_lemma {Γ τ Δ} (L : 𝑳 Δ) (es : NamedEnv (Exp Γ) Δ) (s : Stm Γ τ) :
+    LemmaSem ->
+    ⊢ semWP' (stm_lemmak L es s) ≼ semWP (stm_lemmak L es s).
+  Proof.
+    iIntros (lemSem POST δ) "WPs". specialize (lemSem _ L).
+    unfold semWP. rewrite wp_unfold. cbn.
+    iIntros (σ ns ks1 ks nt) "Hregs".
+    iMod (fupd_mask_subseteq empty) as "Hclose"; first set_solver.
+    iModIntro. iSplitR; [trivial|].
+    iIntros (e3 σ2 efs) "%".
+    dependent elimination H.
+    fold_semWP.
+    dependent elimination s0.
+    iModIntro. iModIntro. iModIntro.
+    iMod "Hclose" as "_".
+    iModIntro; iFrame.
+    iSplitL; [|trivial].
+    unfold semWP'; cbn.
+    rewrite equiv_call_lemma.
+    destruct LEnv as [Σe δΔ req ens]. cbn in lemSem |- *.
+    iDestruct "WPs" as "[% [% [req ens]]]".
+    iApply "ens". by iApply lemSem.
+  Qed.
+
+  Lemma rule_if {Γ τ} (e : Exp Γ ty.bool) (s1 s2 : Stm Γ τ) :
+    ⊢ semWP' (stm_if e s1 s2) ≼ semWP (stm_if e s1 s2).
+  Proof.
+    iIntros (POST δ) "wp". unfold semWP. rewrite wp_unfold. cbn.
+    iIntros (σ _ ks1 ks nt) "Hregs".
+    iMod (fupd_mask_subseteq empty) as "Hclose"; first set_solver.
+    iModIntro. iSplitR; [trivial|].
+    iIntros (e2 σ2 efs) "%".
+    dependent elimination H.
+    fold_semWP.
+    dependent elimination s.
+    iModIntro. iModIntro. iModIntro.
+    iMod "Hclose" as "_".
+    iModIntro; iFrame.
+    iSplitL; [|trivial].
+    unfold semWP'; cbn.
+    now destruct (eval e1 δ1).
+  Qed.
+
+  Lemma rule_seq {Γ τ σ} (s1 : Stm Γ σ) (s2 : Stm Γ τ) :
+    ⊢ semWP' (stm_seq s1 s2) ≼ semWP (stm_seq s1 s2).
+  Proof.
+    iIntros (POST δ) "WPs1". unfold semWP. rewrite wp_unfold. cbn.
+    iIntros ([regs μ] ns ks1 ks nt) "Hregs".
+    iMod (fupd_mask_subseteq empty) as "Hclose"; first set_solver.
+    iModIntro.
+    iSplitR; [trivial|].
+    iIntros (e2 σ2 efs) "%".
+    dependent elimination H.
+    fold_semWP.
+    dependent elimination s.
+    iModIntro. iModIntro. iModIntro.
+    iMod "Hclose" as "_". iFrame.
+    iModIntro.
+    iSplitL; [|trivial].
+    unfold semWP'; cbn.
+    by iApply rule_bind.
+  Qed.
+
+  Lemma rule_assertk {Γ τ} (e1 : Exp Γ ty.bool) (e2 : Exp Γ ty.string) (s : Stm Γ τ) :
+    ⊢ semWP' (stm_assertk e1 e2 s) ≼ semWP (stm_assertk e1 e2 s).
+  Proof.
+    iIntros (POST δ) "WPs". unfold semWP. rewrite wp_unfold. cbn.
+    iIntros (σ ns ks1 ks nt) "Hregs".
+    iMod (fupd_mask_subseteq empty) as "Hclose"; first set_solver.
+    iModIntro. iSplitR; [trivial|].
+    iIntros (e3 σ2 efs) "%".
+    dependent elimination H.
+    fold_semWP.
+    dependent elimination s0.
+    iModIntro. iModIntro. iModIntro.
+    iMod "Hclose" as "_".
+    iModIntro; iFrame.
+    iSplitL; [|trivial].
+    unfold semWP'; cbn.
+    destruct (eval e3 δ1).
+    - by iApply "WPs".
+    - by iApply semWP_fail.
+  Qed.
+
+  Lemma rule_match_list {Γ τ σ xh xt} (e : Exp Γ (ty.list σ))
+    (s1 : Stm Γ τ) (s2 : Stm (Γ ▻ xh∷σ ▻ xt∷ty.list σ) τ) :
+    ⊢ semWP' (stm_match_list e s1 xh xt s2) ≼ semWP (stm_match_list e s1 xh xt s2).
+  Proof.
+    iIntros (POST δ) "WPs". unfold semWP. rewrite wp_unfold. cbn.
+    iIntros (σ1 ns ks1 ks nt) "Hregs".
+    iMod (fupd_mask_subseteq empty) as "Hclose"; first set_solver.
+    iModIntro. iSplitR; [trivial|].
+    iIntros (e3 σ2 efs) "%".
+    dependent elimination H.
+    fold_semWP.
+    dependent elimination s.
+    iModIntro. iModIntro. iModIntro.
+    iMod "Hclose" as "_".
+    iModIntro; iFrame.
+    iSplitL; [|trivial].
+    unfold semWP'; cbn.
+    destruct eval as [|l ls]; [easy|].
+    by iApply (rule_block [env].[xh0∷_ ↦ l].[xt0∷ty.list _ ↦ ls]).
+  Qed.
+
+  Lemma rule_match_sum {Γ τ σinl σinr xinl xinr} (e : Exp Γ (ty.sum σinl σinr))
+    (s1 : Stm (Γ ▻ xinl∷σinl) τ) (s2 : Stm (Γ ▻ xinr∷σinr) τ) :
+    ⊢ semWP' (stm_match_sum e xinl s1 xinr s2) ≼ semWP (stm_match_sum e xinl s1 xinr s2).
+  Proof.
+    iIntros (POST δ) "WPs". unfold semWP. rewrite wp_unfold. cbn.
+    iIntros (σ1 _ ks1 ks nt) "Hregs".
+    iMod (fupd_mask_subseteq empty) as "Hclose"; first set_solver.
+    iModIntro. iSplitR; [trivial|].
+    iIntros (e2 σ2 efs) "%".
+    dependent elimination H.
+    fold_semWP.
+    dependent elimination s.
+    iModIntro. iModIntro. iModIntro.
+    iMod "Hclose" as "_".
+    iModIntro. iFrame.
+    iSplitL; [|trivial].
+    unfold semWP'; cbn.
+    destruct eval.
+    - by iApply (rule_block [env].[xinl0∷σinl0 ↦ v]).
+    - by iApply (rule_block [env].[xinr0∷σinr0 ↦ v]).
+  Qed.
+
+  Lemma rule_match_prod {Γ τ σ1 σ2 xl xr} (e : Exp Γ (ty.prod σ1 σ2)) (s : Stm (Γ▻xl∷σ1▻xr∷σ2) τ) :
+    ⊢ semWP' (stm_match_prod e xl xr s) ≼ semWP (stm_match_prod e xl xr s).
+  Proof.
+    iIntros (POST δ) "WPs". unfold semWP. rewrite wp_unfold. cbn.
+    iIntros (σ _ ks1 ks nt) "Hregs".
+    iMod (fupd_mask_subseteq empty) as "Hclose"; first set_solver.
+    iModIntro. iSplitR; [trivial|].
+    iIntros (e2 σ' efs) "%".
+    dependent elimination H.
+    fold_semWP.
+    dependent elimination s0.
+    iModIntro. iModIntro. iModIntro.
+    iMod "Hclose" as "_".
+    iModIntro. iFrame.
+    iSplitL; [|trivial].
+    unfold semWP'; cbn.
+    destruct eval as [v1 v2].
+    by iApply (rule_block [env].[_∷_ ↦ _].[_∷_ ↦ _]).
+  Qed.
+
+  Lemma rule_match_enum {Γ τ E} (e : Exp Γ (ty.enum E)) (alts : enumt E → Stm Γ τ) :
+    ⊢ semWP' (stm_match_enum E e alts) ≼ semWP (stm_match_enum E e alts).
+  Proof.
+    iIntros (POST δ) "WPa". unfold semWP. rewrite wp_unfold. cbn.
+    iIntros (σ _ ks1 ks nt) "Hregs".
+    iMod (fupd_mask_subseteq empty) as "Hclose"; first set_solver.
+    iModIntro. iSplitR; [trivial|].
+    iIntros (e2 σ' efs) "%".
+    dependent elimination H.
+    fold_semWP.
+    dependent elimination s.
+    iModIntro. iModIntro. iModIntro.
+    iMod "Hclose" as "_".
+    iModIntro. by iFrame.
+  Qed.
+
+  Lemma rule_match_tuple {Γ τ σs Δ} (e : Exp Γ (ty.tuple σs)) (p : TuplePat σs Δ)
+    (s : Stm (Γ ▻▻ Δ) τ) :
+    ⊢ semWP' (stm_match_tuple e p s) ≼ semWP (stm_match_tuple e p s).
+  Proof.
+    iIntros (POST δ) "WPs". unfold semWP. rewrite wp_unfold. cbn.
+    iIntros (σ ns ks1 ks nt) "state_inv".
+    iMod (fupd_mask_subseteq empty) as "Hclose"; first set_solver.
+    iModIntro.
+    iSplitR; [trivial|].
+    iIntros (e2 σ' efs) "%".
+    dependent elimination H.
+    fold_semWP.
+    dependent elimination s0.
+    iModIntro. iModIntro. iModIntro.
+    iMod "Hclose" as "_".
+    iModIntro.
+    iFrame; iSplitL; auto.
+    unfold semWP'; cbn.
+    by iApply rule_block.
+  Qed.
+
+  Lemma rule_match_union {Γ τ U} (e : Exp Γ (ty.union U))
+    (alt__ctx : unionk U → PCtx)
+    (alt__pat : ∀ K : unionk U, Pattern (alt__ctx K) (unionk_ty U K))
+    (alt__rhs : ∀ K : unionk U, Stm (Γ ▻▻ alt__ctx K) τ) :
+    ⊢ semWP' (stm_match_union U e alt__pat alt__rhs) ≼
+      semWP (stm_match_union U e alt__pat alt__rhs).
+  Proof.
+    iIntros (POST δ) "WPs". unfold semWP. rewrite wp_unfold. cbn.
+    iIntros (σ ns ks1 ks nt) "state_inv".
+    iMod (fupd_mask_subseteq empty) as "Hclose"; first set_solver.
+    iModIntro.
+    iSplitR; [trivial|].
+    iIntros (e2 σ' efs) "%".
+    dependent elimination H.
+    fold_semWP.
+    dependent elimination s.
+    iModIntro. iModIntro. iModIntro.
+    iMod "Hclose" as "_".
+    iModIntro.
+    iFrame; iSplitL; auto.
+    unfold semWP'; cbn.
+    destruct unionv_unfold.
+    by iApply rule_block.
+  Qed.
+
+  Lemma rule_match_record {Γ τ R Δ} (e : Exp Γ (ty.record R))
+    (p : RecordPat (recordf_ty R) Δ) (s : Stm (Γ ▻▻ Δ) τ) :
+    ⊢ semWP' (stm_match_record R e p s) ≼
+      semWP (stm_match_record R e p s).
+  Proof.
+    iIntros (POST δ) "WPs". unfold semWP. rewrite wp_unfold. cbn.
+    iIntros (σ ns ks1 ks nt) "state_inv".
+    iMod (fupd_mask_subseteq empty) as "Hclose"; first set_solver.
+    iModIntro.
+    iSplitR; [trivial|].
+    iIntros (e2 σ' efs) "%".
+    dependent elimination H.
+    fold_semWP.
+    dependent elimination s0.
+    iModIntro. iModIntro. iModIntro.
+    iMod "Hclose" as "_".
+    iModIntro.
+    iFrame; iSplitL; auto.
+    unfold semWP'; cbn.
+    by iApply rule_block.
+  Qed.
+
+  Lemma rule_match_bvec {Γ τ n} (e : Exp Γ (ty.bvec n)) (rhs : bv n → Stm Γ τ) :
+    ⊢ semWP' (stm_match_bvec n e rhs) ≼ semWP (stm_match_bvec n e rhs).
+  Proof.
+    iIntros (POST δ) "WPs". unfold semWP. rewrite wp_unfold. cbn.
+    iIntros (σ ns ks1 ks nt) "state_inv".
+    iMod (fupd_mask_subseteq empty) as "Hclose"; first set_solver.
+    iModIntro.
+    iSplitR; [trivial|].
+    iIntros (e2 σ' efs) "%".
+    dependent elimination H.
+    fold_semWP.
+    dependent elimination s.
+    iModIntro. iModIntro. iModIntro.
+    iMod "Hclose" as "_".
+    iModIntro. by iFrame.
+  Qed.
+
+  Lemma rule_match_bvec_split {Γ τ m n xl xr} (e : Exp Γ (ty.bvec (m + n)))
+    (s : Stm (Γ ▻ xl∷ty.bvec m ▻ xr∷ty.bvec n) τ) :
+    ⊢ semWP' (stm_match_bvec_split m n e xl xr s) ≼
+      semWP (stm_match_bvec_split m n e xl xr s).
+  Proof.
+    iIntros (POST δ) "WPs". unfold semWP. rewrite wp_unfold. cbn.
+    iIntros (σ ns ks1 ks nt) "state_inv".
+    iMod (fupd_mask_subseteq empty) as "Hclose"; first set_solver.
+    iModIntro.
+    iSplitR; [trivial|].
+    iIntros (e2 σ' efs) "%".
+    dependent elimination H.
+    fold_semWP.
+    dependent elimination s0.
+    iModIntro. iModIntro. iModIntro.
+    iMod "Hclose" as "_".
+    iModIntro.
+    iFrame; iSplitL; auto.
+    unfold semWP'; cbn.
+    destruct bv.appView.
+    by iApply (rule_block [env].[_∷ty.bvec m0 ↦ xs].[_∷ty.bvec n1 ↦ ys]).
+  Qed.
+
+  Lemma rule_read_register {Γ τ} (reg : 𝑹𝑬𝑮 τ) :
+    ⊢ semWP' (Γ := Γ) (stm_read_register reg) ≼ semWP (stm_read_register reg).
+  Proof.
+    iIntros (POST δ) "[% [Hreg HP]]"; cbn.
+    unfold semWP. iApply (wp_mask_mono _ empty); auto.
+    rewrite wp_unfold; cbn.
+    iIntros (σ _ ls _ n) "[Hregs Hmem]".
+    iDestruct (@reg_valid with "Hregs Hreg") as %<-.
+    iModIntro.
+    iSplitR; [trivial|].
+    iIntros (e2 σ2 efs) "%".
+    dependent elimination H.
+    dependent elimination s.
+    iModIntro. iModIntro. iModIntro.
+    iFrame. iSplitR ""; auto.
+    iModIntro.
+    iApply wp_value.
+    by iApply "HP".
+  Qed.
+
+  Lemma rule_write_register {Γ τ} (reg : 𝑹𝑬𝑮 τ) (e : Exp Γ τ) :
+    ⊢ semWP' (stm_write_register reg e) ≼ semWP (stm_write_register reg e).
+  Proof.
+    iIntros (POST δ) "[% [Hreg HP]]"; cbn.
+    unfold semWP. iApply (wp_mask_mono _ empty); auto.
+    rewrite wp_unfold; cbn.
+    iIntros (σ _ ls _ n) "[Hregs Hmem]".
+    iMod (reg_update σ.1 reg v (eval e δ) with "Hregs Hreg") as "[Hregs Hreg]".
+    iModIntro.
+    iSplitR; [trivial|].
+    iIntros (e2 σ2 efs) "%".
+    dependent elimination H.
+    destruct (steps_inversion_write_register s) as [-> [<- [<- ->]]].
+    iModIntro. iModIntro. iModIntro.
+    iFrame. iSplitL; auto.
+    iApply wp_value.
+    by iApply "HP".
+  Qed.
+
+  Lemma rule_debug {Γ τ} (s : Stm Γ τ) :
+    ⊢ semWP' (stm_debugk s) ≼ semWP (stm_debugk s).
+  Proof.
+    iIntros (POST δ) "WPs". unfold semWP. rewrite wp_unfold. cbn.
+    iIntros (σ ns ks1 ks nt) "Hregs".
+    iMod (fupd_mask_subseteq empty) as "Hclose"; first set_solver.
+    iModIntro. iSplitR; [trivial|].
+    iIntros (e3 σ2 efs) "%".
+    dependent elimination H.
+    fold_semWP.
+    dependent elimination s0.
+    iModIntro. iModIntro. iModIntro.
+    iMod "Hclose" as "_".
+    iModIntro; by iFrame.
+  Qed.
+
+  Lemma sound_stm_open (extSem : ForeignSem) (lemSem : LemmaSem) :
+    forall {Γ τ} (s : Stm Γ τ),
+      ⊢ semWP' s ≼ semWP s.
+  Proof.
+    unfold semWP', ref.
+    intros Γ τ [].
+    - apply rule_val.
+    - cbn.
+      apply rule_exp.
+    - apply rule_let.
+    - apply rule_block.
+    - apply rule_assign.
+    - apply rule_call; auto.
+    - apply rule_call_frame.
+    - apply rule_foreign; auto.
+    - apply rule_lemma; auto.
+    - apply rule_if.
+    - apply rule_seq.
+    - cbn.
+      apply rule_assertk.
+    - apply rule_fail.
+    - admit.
+    - cbn. apply rule_match_list.
+    - cbn. apply rule_match_sum.
+    - cbn. apply rule_match_enum.
+    - cbn. apply rule_match_tuple.
+    - cbn. apply rule_match_union.
+    - cbn. apply rule_match_record.
+    - cbn. apply rule_match_bvec.
+    - cbn. apply rule_match_bvec_split.
+    - apply rule_read_register.
+    - cbn. apply rule_write_register.
+    - apply rule_bind.
+    - apply rule_debug.
+  Admitted.
+
+  Lemma sound_stm (extSem : ForeignSem) (lemSem : LemmaSem) :
+    forall {Γ τ} (s : Stm Γ τ) (Q : Val τ → CStore Γ → iProp Σ) (δ : CStore Γ),
+      CHeapSpecM.exec_aux semCall s Q δ ⊢ semWP s Q δ.
+  Proof.
+    intros.
+    apply (CHeapSpecM.fold_exec_aux (ex := semWP) (ec := semCall)).
+    - admit.
+    - clear - extSem lemSem.
+      intros Γ τ s.
+      intros P Q PQ δ. cbn.
+      iIntros "WP". iApply sound_stm_open; auto.
+      unfold semWP'.
+      iStopProof.
+      iApply CHeapSpecM.exec_open_monotonic; auto.
+      admit.
+      admit.
+    - unfold pointwise_relation. easy.
+  Admitted.
+
+  Import sep.instances.
+
+  Lemma sound :
+    ForeignSem -> LemmaSem -> Shallow.ValidContractCEnv ->
+    ⊢ Shallow.ValidContractEnvSem semWP.
+  Proof.
+    intros extSem lemSem vcenv.
+    iLöb as "IH".
+    iIntros (σs σ f).
+    specialize (vcenv σs σ f).
+    destruct (CEnv f) as [[Σe δΔ req res ens]|];[|trivial].
+    iIntros (ι) "PRE".
+    specialize (vcenv _ eq_refl).
+    cbn in vcenv.
+    rewrite env.Forall_forall in vcenv.
+    specialize (vcenv ι).
+    rewrite CPureSpecM.wp_produce in vcenv.
+    cbn in vcenv.
+    iPoseProof (vcenv with "[$] PRE") as "vcenv". clear vcenv.
+    iApply (sound_stm extSem lemSem).
+    iRevert "vcenv".
+    iApply CHeapSpecM.exec_aux_monotonic.
+  Abort.
+
+  End WithSailGS.
+
+End IrisInstanceWithContracts.
